CoqOfRust/ink/ink_env.v
@@ -427,6 +427,361 @@ Definition Gas : Set := u64.
 
 Definition BlockNumber : Set := u32.
 
+Module contract.
+  Module ContractEnv.
+    Class Trait (Self : Set) : Type := {
+      Env : Set;
+      _ : exists `(ink_env.types.Environment.Trait Env), True;
+    }.
+    
+    Global Instance Method_Env `(Trait)
+      : Notation.DoubleColonType Self "Env" := {
+      Notation.double_colon_type := Env;
+    }.
+  End ContractEnv.
+  
+  Module ContractReference.
+    Class Trait (Self : Set) : Type := {
+      Type_ : Set;
+    }.
+    
+    Global Instance Method_Type_ `(Trait)
+      : Notation.DoubleColonType Self "Type_" := {
+      Notation.double_colon_type := Type_;
+    }.
+  End ContractReference.
+End contract.
+
+Module call.
+  Module common.
+    Module ReturnType.
+      Section ReturnType.
+        Context {T : Set}.
+        Unset Primitive Projections.
+        Record t : Set := {
+          _ : core.marker.PhantomData (T);
+        }.
+        Global Set Primitive Projections.
+        
+        Global Instance Get_0 : Notation.Dot 0 := {
+          Notation.dot '(Build_t x0) := x0;
+        }.
+      End ReturnType.
+    End ReturnType.
+    Definition ReturnType := @ReturnType.t.
+    
+    Module Set_.
+      Section Set_.
+        Context {T : Set}.
+        Unset Primitive Projections.
+        Record t : Set := {
+          _ : T;
+        }.
+        Global Set Primitive Projections.
+        
+        Global Instance Get_0 : Notation.Dot 0 := {
+          Notation.dot '(Build_t x0) := x0;
+        }.
+      End Set_.
+    End Set_.
+    Definition Set_ := @Set_.t.
+    
+    Module Unset_.
+      Section Unset_.
+        Context {T : Set}.
+        Unset Primitive Projections.
+        Record t : Set := {
+          _ : core.marker.PhantomData (T);
+        }.
+        Global Set Primitive Projections.
+        
+        Global Instance Get_0 : Notation.Dot 0 := {
+          Notation.dot '(Build_t x0) := x0;
+        }.
+      End Unset_.
+    End Unset_.
+    Definition Unset_ := @Unset_.t.
+    
+    Module Unwrap.
+      Class Trait (Self : Set) : Type := {
+        Output : Set;
+        unwrap_or_else
+          `{H' : State.Trait}
+          {F: Set}
+          `{H'0 : core.ops.function.FnOnce.Trait F (Args := unit)}
+          :
+          Self -> F -> (M (H := H') Output);
+      }.
+      
+      Global Instance Method_Output `(Trait)
+        : Notation.DoubleColonType Self "Output" := {
+        Notation.double_colon_type := Output;
+      }.
+      Global Instance Method_unwrap_or_else `{H' : State.Trait} `(Trait)
+        : Notation.Dot "unwrap_or_else" := {
+        Notation.dot
+          {F : Set}
+          `{H'0 : core.ops.function.FnOnce.Trait F (Args := unit)}
+          :=
+          unwrap_or_else (F := F) (H'0 := H'0);
+      }.
+    End Unwrap.
+  End common.
+  
+  Module selector.
+    Module Selector.
+      Unset Primitive Projections.
+      Record t : Set := {
+        bytes : list u8;
+      }.
+      Global Set Primitive Projections.
+      
+      Global Instance Get_bytes : Notation.Dot "bytes" := {
+        Notation.dot '(Build_t x0) := x0;
+      }.
+    End Selector.
+    Definition Selector : Set := Selector.t.
+  End selector.
+  
+  Module execution_input.
+    Module ExecutionInput.
+      Section ExecutionInput.
+        Context {Args : Set}.
+        Unset Primitive Projections.
+        Record t : Set := {
+          selector : ink_env.call.selector.Selector;
+          args : Args;
+        }.
+        Global Set Primitive Projections.
+        
+        Global Instance Get_selector : Notation.Dot "selector" := {
+          Notation.dot '(Build_t x0 _) := x0;
+        }.
+        Global Instance Get_args : Notation.Dot "args" := {
+          Notation.dot '(Build_t _ x1) := x1;
+        }.
+      End ExecutionInput.
+    End ExecutionInput.
+    Definition ExecutionInput (Args : Set) : Set :=
+      ExecutionInput.t (Args := Args).
+    
+    Module ArgumentList.
+      Section ArgumentList.
+        Context {Head Rest : Set}.
+        Unset Primitive Projections.
+        Record t : Set := {
+          head : Head;
+          rest : Rest;
+        }.
+        Global Set Primitive Projections.
+        
+        Global Instance Get_head : Notation.Dot "head" := {
+          Notation.dot '(Build_t x0 _) := x0;
+        }.
+        Global Instance Get_rest : Notation.Dot "rest" := {
+          Notation.dot '(Build_t _ x1) := x1;
+        }.
+      End ArgumentList.
+    End ArgumentList.
+    Definition ArgumentList (Head Rest : Set) : Set :=
+      ArgumentList.t (Head := Head) (Rest := Rest).
+    
+    Module Argument.
+      Section Argument.
+        Context {T : Set}.
+        Unset Primitive Projections.
+        Record t : Set := {
+          arg : T;
+        }.
+        Global Set Primitive Projections.
+        
+        Global Instance Get_arg : Notation.Dot "arg" := {
+          Notation.dot '(Build_t x0) := x0;
+        }.
+      End Argument.
+    End Argument.
+    Definition Argument (T : Set) : Set := Argument.t (T := T).
+    
+    Definition ArgsList (Head Rest : Set) : Set :=
+      ink_env.call.execution_input.ArgumentList
+        (ink_env.call.execution_input.Argument Head)
+        Rest.
+    
+    Module ArgumentListEnd.
+      Inductive t : Set := Build.
+    End ArgumentListEnd.
+    Definition ArgumentListEnd := @ArgumentListEnd.t.
+    
+    Definition EmptyArgumentList : Set :=
+      ink_env.call.execution_input.ArgumentList
+        ink_env.call.execution_input.ArgumentListEnd
+        ink_env.call.execution_input.ArgumentListEnd.
+  End execution_input.
+  
+  Module create_builder.
+    Module state.
+      Module Salt.
+        Inductive t : Set :=
+        .
+      End Salt.
+      Definition Salt := Salt.t.
+    End state.
+    
+    Module FromAccountId.
+      Class Trait
+          (Self : Set) {T : Set} `{ink_env.types.Environment.Trait T} :
+          Type := {
+        from_account_id
+          `{H' : State.Trait}
+          :
+          ink_env.types.Environment.AccountId -> (M (H := H') Self);
+      }.
+      
+      Global Instance Method_from_account_id `{H' : State.Trait} `(Trait)
+        : Notation.Dot "from_account_id" := {
+        Notation.dot := from_account_id;
+      }.
+    End FromAccountId.
+    
+    Module ConstructorReturnType.
+      Class Trait (Self : Set) {C : Set} : Type := {
+        IS_RESULT `{H' : State.Trait} : bool;
+        Output : Set;
+        Error : Set;
+        _ : exists `(parity_scale_codec.codec.Decode.Trait Error), True;
+        ok `{H' : State.Trait} : C -> (M (H := H') Output);
+      }.
+      
+      Global Instance Method_IS_RESULT `{H' : State.Trait} `(Trait)
+        : Notation.Dot "IS_RESULT" := {
+        Notation.dot := IS_RESULT;
+      }.
+      Global Instance Method_Output `(Trait)
+        : Notation.DoubleColonType Self "Output" := {
+        Notation.double_colon_type := Output;
+      }.
+      Global Instance Method_Error `(Trait)
+        : Notation.DoubleColonType Self "Error" := {
+        Notation.double_colon_type := Error;
+      }.
+      Global Instance Method_ok `{H' : State.Trait} `(Trait)
+        : Notation.Dot "ok" := {
+        Notation.dot := ok;
+      }.
+      Global Instance Method_err `{H' : State.Trait} `(Trait)
+        : Notation.Dot "err" := {
+        Notation.dot (_err : Error)
+          :=
+          (axiom : M (H := H') (core.option.Option Output));
+      }.
+    End ConstructorReturnType.
+    
+    Module CreateParams.
+      Section CreateParams.
+        Context {E ContractRef Args Salt R : Set}.
+        Context `{ink_env.types.Environment.Trait E}.
+        Unset Primitive Projections.
+        Record t : Set := {
+          code_hash : E::type["Hash"];
+          gas_limit : u64;
+          endowment : E::type["Balance"];
+          exec_input : ink_env.call.execution_input.ExecutionInput Args;
+          salt_bytes : Salt;
+          _return_type : ink_env.call.common.ReturnType R;
+          _phantom : core.marker.PhantomData (ContractRef);
+        }.
+        Global Set Primitive Projections.
+        
+        Global Instance Get_code_hash : Notation.Dot "code_hash" := {
+          Notation.dot '(Build_t x0 _ _ _ _ _ _) := x0;
+        }.
+        Global Instance Get_gas_limit : Notation.Dot "gas_limit" := {
+          Notation.dot '(Build_t _ x1 _ _ _ _ _) := x1;
+        }.
+        Global Instance Get_endowment : Notation.Dot "endowment" := {
+          Notation.dot '(Build_t _ _ x2 _ _ _ _) := x2;
+        }.
+        Global Instance Get_exec_input : Notation.Dot "exec_input" := {
+          Notation.dot '(Build_t _ _ _ x3 _ _ _) := x3;
+        }.
+        Global Instance Get_salt_bytes : Notation.Dot "salt_bytes" := {
+          Notation.dot '(Build_t _ _ _ _ x4 _ _) := x4;
+        }.
+        Global Instance Get__return_type : Notation.Dot "_return_type" := {
+          Notation.dot '(Build_t _ _ _ _ _ x5 _) := x5;
+        }.
+        Global Instance Get__phantom : Notation.Dot "_phantom" := {
+          Notation.dot '(Build_t _ _ _ _ _ _ x6) := x6;
+        }.
+      End CreateParams.
+    End CreateParams.
+    Definition CreateParams
+        (E ContractRef Args Salt R : Set)
+        `{ink_env.types.Environment.Trait E}
+        : Set :=
+      CreateParams.t
+        (E := E)
+        (ContractRef := ContractRef)
+        (Args := Args)
+        (Salt := Salt)
+        (R := R).
+    
+    Module CreateBuilder.
+      Section CreateBuilder.
+        Context
+          {E ContractRef CodeHash GasLimit Endowment Args Salt RetType : Set}.
+        Context `{ink_env.types.Environment.Trait E}.
+        Unset Primitive Projections.
+        Record t : Set := {
+          code_hash : CodeHash;
+          gas_limit : GasLimit;
+          endowment : Endowment;
+          exec_input : Args;
+          salt : Salt;
+          return_type : RetType;
+          _phantom : core.marker.PhantomData (E * ContractRef);
+        }.
+        Global Set Primitive Projections.
+        
+        Global Instance Get_code_hash : Notation.Dot "code_hash" := {
+          Notation.dot '(Build_t x0 _ _ _ _ _ _) := x0;
+        }.
+        Global Instance Get_gas_limit : Notation.Dot "gas_limit" := {
+          Notation.dot '(Build_t _ x1 _ _ _ _ _) := x1;
+        }.
+        Global Instance Get_endowment : Notation.Dot "endowment" := {
+          Notation.dot '(Build_t _ _ x2 _ _ _ _) := x2;
+        }.
+        Global Instance Get_exec_input : Notation.Dot "exec_input" := {
+          Notation.dot '(Build_t _ _ _ x3 _ _ _) := x3;
+        }.
+        Global Instance Get_salt : Notation.Dot "salt" := {
+          Notation.dot '(Build_t _ _ _ _ x4 _ _) := x4;
+        }.
+        Global Instance Get_return_type : Notation.Dot "return_type" := {
+          Notation.dot '(Build_t _ _ _ _ _ x5 _) := x5;
+        }.
+        Global Instance Get__phantom : Notation.Dot "_phantom" := {
+          Notation.dot '(Build_t _ _ _ _ _ _ x6) := x6;
+        }.
+      End CreateBuilder.
+    End CreateBuilder.
+    Definition CreateBuilder
+        (E ContractRef CodeHash GasLimit Endowment Args Salt RetType : Set)
+        `{ink_env.types.Environment.Trait E}
+        : Set :=
+      CreateBuilder.t
+        (E := E)
+        (ContractRef := ContractRef)
+        (CodeHash := CodeHash)
+        (GasLimit := GasLimit)
+        (Endowment := Endowment)
+        (Args := Args)
+        (Salt := Salt)
+        (RetType := RetType).
+  End create_builder.
+End call.
+
 Module engine.
   Module off_chain.
     Module call_data.
@@ -658,7 +1013,7 @@ Module topics.
       push_topic
         `{H' : State.Trait}
         {T: Set}
-        `{parity_scale_codec.codec.Encode.Trait T}
+        `{H'0 : parity_scale_codec.codec.Encode.Trait T}
         :
         (mut_ref Self) -> (ref T) -> (M (H := H') unit);
       output `{H' : State.Trait} : Self -> (M (H := H') Output);
@@ -674,9 +1029,9 @@ Module topics.
     }.
     Global Instance Method_push_topic `{H' : State.Trait} `(Trait)
       : Notation.Dot "push_topic" := {
-      Notation.dot {T : Set} `{parity_scale_codec.codec.Encode.Trait T}
+      Notation.dot {T : Set} `{H'0 : parity_scale_codec.codec.Encode.Trait T}
         :=
-        push_topic;
+        push_topic (T := T) (H'0 := H'0);
     }.
     Global Instance Method_output `{H' : State.Trait} `(Trait)
       : Notation.Dot "output" := {
@@ -758,8 +1113,8 @@ Module topics.
       topics
         `{H' : State.Trait}
         {E B: Set}
-        `{ink_env.types.Environment.Trait E}
-        `{ink_env.topics.TopicsBuilderBackend.Trait B (E := E)}
+        `{H'0 : ink_env.types.Environment.Trait E}
+        `{H'1 : ink_env.topics.TopicsBuilderBackend.Trait B (E := E)}
         :
         (ref Self) ->
         (ink_env.topics.TopicsBuilder ink_env.topics.state.Uninit E B) ->
@@ -774,10 +1129,10 @@ Module topics.
       : Notation.Dot "topics" := {
       Notation.dot
         {E B : Set}
-        `{ink_env.types.Environment.Trait E}
-        `{ink_env.topics.TopicsBuilderBackend.Trait B (E := E)}
+        `{H'0 : ink_env.types.Environment.Trait E}
+        `{H'1 : ink_env.topics.TopicsBuilderBackend.Trait B (E := E)}
         :=
-        topics;
+        topics (E := E) (B := B) (H'0 := H'0) (H'1 := H'1);
     }.
   End Topics.
   
@@ -801,29 +1156,6 @@ Module topics.
   End PrefixedValue.
   Definition PrefixedValue (T : Set) : Set := PrefixedValue.t (T := T).
 End topics.
-
-Module error.
-  Module Error.
-    Inductive t : Set :=
-    | Decode (_ : parity_scale_codec.error.Error)
-    | OffChain (_ : ink_env.engine.off_chain.OffChainError)
-    | CalleeTrapped
-    | CalleeReverted
-    | KeyNotFound
-    | _BelowSubsistenceThreshold
-    | TransferFailed
-    | _EndowmentTooLow
-    | CodeNotFound
-    | NotCallable
-    | Unknown
-    | LoggingDisabled
-    | CallRuntimeFailed
-    | EcdsaRecoveryFailed.
-  End Error.
-  Definition Error := Error.t.
-  
-  Definition Result (T : Set) : Set := core.result.Result T ink_env.error.Error.
-End error.
 
 Module hash.
   Module private.
@@ -894,19 +1226,28 @@ Module hash.
   Definition Blake2x128 := Blake2x128.t.
 End hash.
 
-Module backend.
-  Module ReturnFlags.
-    Unset Primitive Projections.
-    Record t : Set := {
-      value : u32;
-    }.
-    Global Set Primitive Projections.
-    
-    Global Instance Get_value : Notation.Dot "value" := {
-      Notation.dot '(Build_t x0) := x0;
-    }.
-  End ReturnFlags.
-  Definition ReturnFlags : Set := ReturnFlags.t.
+Module backend_and_call_builder_and_error.
+  Module Error.
+    Inductive t : Set :=
+    | Decode (_ : parity_scale_codec.error.Error)
+    | OffChain (_ : ink_env.engine.off_chain.OffChainError)
+    | CalleeTrapped
+    | CalleeReverted
+    | KeyNotFound
+    | _BelowSubsistenceThreshold
+    | TransferFailed
+    | _EndowmentTooLow
+    | CodeNotFound
+    | NotCallable
+    | Unknown
+    | LoggingDisabled
+    | CallRuntimeFailed
+    | EcdsaRecoveryFailed.
+  End Error.
+  Definition Error := Error.t.
+  
+  Definition Result (T : Set) : Set :=
+    core.result.Result T ink_env.backend_and_call_builder_and_error.Error.
   
   Module CallFlags.
     Unset Primitive Projections.
@@ -933,13 +1274,164 @@ Module backend.
   End CallFlags.
   Definition CallFlags : Set := CallFlags.t.
   
+  Module CallParams.
+    Section CallParams.
+      Context {E CallType Args R : Set}.
+      Context `{ink_env.types.Environment.Trait E}.
+      Unset Primitive Projections.
+      Record t : Set := {
+        call_type : CallType;
+        call_flags : ink_env.backend_and_call_builder_and_error.CallFlags;
+        _return_type : ink_env.call.common.ReturnType R;
+        exec_input : ink_env.call.execution_input.ExecutionInput Args;
+        _phantom : core.marker.PhantomData (E);
+      }.
+      Global Set Primitive Projections.
+      
+      Global Instance Get_call_type : Notation.Dot "call_type" := {
+        Notation.dot '(Build_t x0 _ _ _ _) := x0;
+      }.
+      Global Instance Get_call_flags : Notation.Dot "call_flags" := {
+        Notation.dot '(Build_t _ x1 _ _ _) := x1;
+      }.
+      Global Instance Get__return_type : Notation.Dot "_return_type" := {
+        Notation.dot '(Build_t _ _ x2 _ _) := x2;
+      }.
+      Global Instance Get_exec_input : Notation.Dot "exec_input" := {
+        Notation.dot '(Build_t _ _ _ x3 _) := x3;
+      }.
+      Global Instance Get__phantom : Notation.Dot "_phantom" := {
+        Notation.dot '(Build_t _ _ _ _ x4) := x4;
+      }.
+    End CallParams.
+  End CallParams.
+  Definition CallParams
+      (E CallType Args R : Set)
+      `{ink_env.types.Environment.Trait E}
+      : Set :=
+    CallParams.t (E := E) (CallType := CallType) (Args := Args) (R := R).
+  
+  Module Call.
+    Section Call.
+      Context {E : Set}.
+      Context `{ink_env.types.Environment.Trait E}.
+      Unset Primitive Projections.
+      Record t : Set := {
+        callee : E::type["AccountId"];
+        gas_limit : ink_env.types.Gas;
+        transferred_value : E::type["Balance"];
+      }.
+      Global Set Primitive Projections.
+      
+      Global Instance Get_callee : Notation.Dot "callee" := {
+        Notation.dot '(Build_t x0 _ _) := x0;
+      }.
+      Global Instance Get_gas_limit : Notation.Dot "gas_limit" := {
+        Notation.dot '(Build_t _ x1 _) := x1;
+      }.
+      Global Instance Get_transferred_value
+        : Notation.Dot "transferred_value" := {
+        Notation.dot '(Build_t _ _ x2) := x2;
+      }.
+    End Call.
+  End Call.
+  Definition Call (E : Set) `{ink_env.types.Environment.Trait E} : Set :=
+    Call.t (E := E).
+  
+  Module CallBuilder.
+    Section CallBuilder.
+      Context {E CallType Args RetType : Set}.
+      Context `{ink_env.types.Environment.Trait E}.
+      Unset Primitive Projections.
+      Record t : Set := {
+        call_type : CallType;
+        call_flags : ink_env.backend_and_call_builder_and_error.CallFlags;
+        exec_input : Args;
+        return_type : RetType;
+        _phantom : core.marker.PhantomData (E);
+      }.
+      Global Set Primitive Projections.
+      
+      Global Instance Get_call_type : Notation.Dot "call_type" := {
+        Notation.dot '(Build_t x0 _ _ _ _) := x0;
+      }.
+      Global Instance Get_call_flags : Notation.Dot "call_flags" := {
+        Notation.dot '(Build_t _ x1 _ _ _) := x1;
+      }.
+      Global Instance Get_exec_input : Notation.Dot "exec_input" := {
+        Notation.dot '(Build_t _ _ x2 _ _) := x2;
+      }.
+      Global Instance Get_return_type : Notation.Dot "return_type" := {
+        Notation.dot '(Build_t _ _ _ x3 _) := x3;
+      }.
+      Global Instance Get__phantom : Notation.Dot "_phantom" := {
+        Notation.dot '(Build_t _ _ _ _ x4) := x4;
+      }.
+    End CallBuilder.
+  End CallBuilder.
+  Definition CallBuilder
+      (E CallType Args RetType : Set)
+      `{ink_env.types.Environment.Trait E}
+      : Set :=
+    CallBuilder.t
+      (E := E)
+      (CallType := CallType)
+      (Args := Args)
+      (RetType := RetType).
+  
+  Parameter build_call :
+      forall `{H' : State.Trait} {E : Set} `{ink_env.types.Environment.Trait E},
+      M (H := H')
+          (ink_env.backend_and_call_builder_and_error.CallBuilder
+            E
+            (ink_env.call.common.Unset_
+              (ink_env.backend_and_call_builder_and_error.Call E))
+            (ink_env.call.common.Unset_
+              (ink_env.call.execution_input.ExecutionInput
+                ink_env.call.execution_input.EmptyArgumentList))
+            (ink_env.call.common.Unset_ (ink_env.call.common.ReturnType unit))).
+  
+  Module DelegateCall.
+    Section DelegateCall.
+      Context {E : Set}.
+      Context `{ink_env.types.Environment.Trait E}.
+      Unset Primitive Projections.
+      Record t : Set := {
+        code_hash : E::type["Hash"];
+      }.
+      Global Set Primitive Projections.
+      
+      Global Instance Get_code_hash : Notation.Dot "code_hash" := {
+        Notation.dot '(Build_t x0) := x0;
+      }.
+    End DelegateCall.
+  End DelegateCall.
+  Definition DelegateCall
+      (E : Set)
+      `{ink_env.types.Environment.Trait E}
+      : Set :=
+    DelegateCall.t (E := E).
+  
+  Module ReturnFlags.
+    Unset Primitive Projections.
+    Record t : Set := {
+      value : u32;
+    }.
+    Global Set Primitive Projections.
+    
+    Global Instance Get_value : Notation.Dot "value" := {
+      Notation.dot '(Build_t x0) := x0;
+    }.
+  End ReturnFlags.
+  Definition ReturnFlags : Set := ReturnFlags.t.
+  
   Module EnvBackend.
     Class Trait (Self : Set) : Type := {
       set_contract_storage
         `{H' : State.Trait}
         {K V: Set}
-        `{parity_scale_codec.codec.Encode.Trait K}
-        `{ink_storage_traits.storage.Storable.Trait V}
+        `{H'0 : parity_scale_codec.codec.Encode.Trait K}
+        `{H'1 : ink_storage_traits.storage.Storable.Trait V}
         :
         (mut_ref Self) ->
         (ref K) ->
@@ -948,46 +1440,51 @@ Module backend.
       get_contract_storage
         `{H' : State.Trait}
         {K R: Set}
-        `{parity_scale_codec.codec.Encode.Trait K}
-        `{ink_storage_traits.storage.Storable.Trait R}
+        `{H'0 : parity_scale_codec.codec.Encode.Trait K}
+        `{H'1 : ink_storage_traits.storage.Storable.Trait R}
         :
         (mut_ref Self) ->
         (ref K) ->
-        (M (H := H') (ink_env.error.Result (core.option.Option R)));
+        (M (H := H')
+          (ink_env.backend_and_call_builder_and_error.Result
+            (core.option.Option R)));
       take_contract_storage
         `{H' : State.Trait}
         {K R: Set}
-        `{parity_scale_codec.codec.Encode.Trait K}
-        `{ink_storage_traits.storage.Storable.Trait R}
+        `{H'0 : parity_scale_codec.codec.Encode.Trait K}
+        `{H'1 : ink_storage_traits.storage.Storable.Trait R}
         :
         (mut_ref Self) ->
         (ref K) ->
-        (M (H := H') (ink_env.error.Result (core.option.Option R)));
+        (M (H := H')
+          (ink_env.backend_and_call_builder_and_error.Result
+            (core.option.Option R)));
       contains_contract_storage
         `{H' : State.Trait}
         {K: Set}
-        `{parity_scale_codec.codec.Encode.Trait K}
+        `{H'0 : parity_scale_codec.codec.Encode.Trait K}
         :
         (mut_ref Self) -> (ref K) -> (M (H := H') (core.option.Option u32));
       clear_contract_storage
         `{H' : State.Trait}
         {K: Set}
-        `{parity_scale_codec.codec.Encode.Trait K}
+        `{H'0 : parity_scale_codec.codec.Encode.Trait K}
         :
         (mut_ref Self) -> (ref K) -> (M (H := H') (core.option.Option u32));
       decode_input
         `{H' : State.Trait}
         {T: Set}
-        `{parity_scale_codec.codec.Decode.Trait T}
+        `{H'0 : parity_scale_codec.codec.Decode.Trait T}
         :
-        (mut_ref Self) -> (M (H := H') (ink_env.error.Result T));
+        (mut_ref Self) ->
+        (M (H := H') (ink_env.backend_and_call_builder_and_error.Result T));
       return_value
         `{H' : State.Trait}
         {R: Set}
-        `{parity_scale_codec.codec.Encode.Trait R}
+        `{H'0 : parity_scale_codec.codec.Encode.Trait R}
         :
         (mut_ref Self) ->
-        ink_env.backend.ReturnFlags ->
+        ink_env.backend_and_call_builder_and_error.ReturnFlags ->
         (ref R) ->
         (M (H := H') Empty_set);
       debug_message
@@ -997,7 +1494,7 @@ Module backend.
       hash_bytes
         `{H' : State.Trait}
         {H: Set}
-        `{ink_env.hash.CryptoHash.Trait H}
+        `{H'0 : ink_env.hash.CryptoHash.Trait H}
         :
         (mut_ref Self) ->
         (ref (Slice u8)) ->
@@ -1006,8 +1503,8 @@ Module backend.
       hash_encoded
         `{H' : State.Trait}
         {H T: Set}
-        `{ink_env.hash.CryptoHash.Trait H}
-        `{parity_scale_codec.codec.Encode.Trait T}
+        `{H'0 : ink_env.hash.CryptoHash.Trait H}
+        `{H'1 : parity_scale_codec.codec.Encode.Trait T}
         :
         (mut_ref Self) ->
         (ref T) ->
@@ -1020,22 +1517,22 @@ Module backend.
         (ref (list u8)) ->
         (ref (list u8)) ->
         (mut_ref (list u8)) ->
-        (M (H := H') (ink_env.error.Result unit));
+        (M (H := H') (ink_env.backend_and_call_builder_and_error.Result unit));
       ecdsa_to_eth_address
         `{H' : State.Trait}
         :
         (mut_ref Self) ->
         (ref (list u8)) ->
         (mut_ref (list u8)) ->
-        (M (H := H') (ink_env.error.Result unit));
+        (M (H := H') (ink_env.backend_and_call_builder_and_error.Result unit));
       call_chain_extension
         `{H' : State.Trait}
         {I T E ErrorCode F D: Set}
-        `{parity_scale_codec.codec.Encode.Trait I}
-        `{parity_scale_codec.codec.Decode.Trait T}
-        `{core.convert.From.Trait E (T := ErrorCode)}
-        `{core.ops.function.FnOnce.Trait F (Args := u32)}
-        `{core.ops.function.FnOnce.Trait D (Args := ref (Slice u8))}
+        `{H'0 : parity_scale_codec.codec.Encode.Trait I}
+        `{H'1 : parity_scale_codec.codec.Decode.Trait T}
+        `{H'2 : core.convert.From.Trait E (T := ErrorCode)}
+        `{H'3 : core.ops.function.FnOnce.Trait F (Args := u32)}
+        `{H'4 : core.ops.function.FnOnce.Trait D (Args := ref (Slice u8))}
         :
         (mut_ref Self) ->
         u32 ->
@@ -1048,62 +1545,62 @@ Module backend.
         :
         (mut_ref Self) ->
         (ref (Slice u8)) ->
-        (M (H := H') (ink_env.error.Result unit));
+        (M (H := H') (ink_env.backend_and_call_builder_and_error.Result unit));
     }.
     
     Global Instance Method_set_contract_storage `{H' : State.Trait} `(Trait)
       : Notation.Dot "set_contract_storage" := {
       Notation.dot
         {K V : Set}
-        `{parity_scale_codec.codec.Encode.Trait K}
-        `{ink_storage_traits.storage.Storable.Trait V}
+        `{H'0 : parity_scale_codec.codec.Encode.Trait K}
+        `{H'1 : ink_storage_traits.storage.Storable.Trait V}
         :=
-        set_contract_storage;
+        set_contract_storage (K := K) (V := V) (H'0 := H'0) (H'1 := H'1);
     }.
     Global Instance Method_get_contract_storage `{H' : State.Trait} `(Trait)
       : Notation.Dot "get_contract_storage" := {
       Notation.dot
         {K R : Set}
-        `{parity_scale_codec.codec.Encode.Trait K}
-        `{ink_storage_traits.storage.Storable.Trait R}
+        `{H'0 : parity_scale_codec.codec.Encode.Trait K}
+        `{H'1 : ink_storage_traits.storage.Storable.Trait R}
         :=
-        get_contract_storage;
+        get_contract_storage (K := K) (R := R) (H'0 := H'0) (H'1 := H'1);
     }.
     Global Instance Method_take_contract_storage `{H' : State.Trait} `(Trait)
       : Notation.Dot "take_contract_storage" := {
       Notation.dot
         {K R : Set}
-        `{parity_scale_codec.codec.Encode.Trait K}
-        `{ink_storage_traits.storage.Storable.Trait R}
+        `{H'0 : parity_scale_codec.codec.Encode.Trait K}
+        `{H'1 : ink_storage_traits.storage.Storable.Trait R}
         :=
-        take_contract_storage;
+        take_contract_storage (K := K) (R := R) (H'0 := H'0) (H'1 := H'1);
     }.
     Global Instance
         Method_contains_contract_storage
         `{H' : State.Trait}
         `(Trait)
       : Notation.Dot "contains_contract_storage" := {
-      Notation.dot {K : Set} `{parity_scale_codec.codec.Encode.Trait K}
+      Notation.dot {K : Set} `{H'0 : parity_scale_codec.codec.Encode.Trait K}
         :=
-        contains_contract_storage;
+        contains_contract_storage (K := K) (H'0 := H'0);
     }.
     Global Instance Method_clear_contract_storage `{H' : State.Trait} `(Trait)
       : Notation.Dot "clear_contract_storage" := {
-      Notation.dot {K : Set} `{parity_scale_codec.codec.Encode.Trait K}
+      Notation.dot {K : Set} `{H'0 : parity_scale_codec.codec.Encode.Trait K}
         :=
-        clear_contract_storage;
+        clear_contract_storage (K := K) (H'0 := H'0);
     }.
     Global Instance Method_decode_input `{H' : State.Trait} `(Trait)
       : Notation.Dot "decode_input" := {
-      Notation.dot {T : Set} `{parity_scale_codec.codec.Decode.Trait T}
+      Notation.dot {T : Set} `{H'0 : parity_scale_codec.codec.Decode.Trait T}
         :=
-        decode_input;
+        decode_input (T := T) (H'0 := H'0);
     }.
     Global Instance Method_return_value `{H' : State.Trait} `(Trait)
       : Notation.Dot "return_value" := {
-      Notation.dot {R : Set} `{parity_scale_codec.codec.Encode.Trait R}
+      Notation.dot {R : Set} `{H'0 : parity_scale_codec.codec.Encode.Trait R}
         :=
-        return_value;
+        return_value (R := R) (H'0 := H'0);
     }.
     Global Instance Method_debug_message `{H' : State.Trait} `(Trait)
       : Notation.Dot "debug_message" := {
@@ -1111,16 +1608,18 @@ Module backend.
     }.
     Global Instance Method_hash_bytes `{H' : State.Trait} `(Trait)
       : Notation.Dot "hash_bytes" := {
-      Notation.dot {H : Set} `{ink_env.hash.CryptoHash.Trait H} := hash_bytes;
+      Notation.dot {H : Set} `{H'0 : ink_env.hash.CryptoHash.Trait H}
+        :=
+        hash_bytes (H := H) (H'0 := H'0);
     }.
     Global Instance Method_hash_encoded `{H' : State.Trait} `(Trait)
       : Notation.Dot "hash_encoded" := {
       Notation.dot
         {H T : Set}
-        `{ink_env.hash.CryptoHash.Trait H}
-        `{parity_scale_codec.codec.Encode.Trait T}
+        `{H'0 : ink_env.hash.CryptoHash.Trait H}
+        `{H'1 : parity_scale_codec.codec.Encode.Trait T}
         :=
-        hash_encoded;
+        hash_encoded (H := H) (T := T) (H'0 := H'0) (H'1 := H'1);
     }.
     Global Instance Method_ecdsa_recover `{H' : State.Trait} `(Trait)
       : Notation.Dot "ecdsa_recover" := {
@@ -1134,518 +1633,380 @@ Module backend.
       : Notation.Dot "call_chain_extension" := {
       Notation.dot
         {I T E ErrorCode F D : Set}
-        `{parity_scale_codec.codec.Encode.Trait I}
-        `{parity_scale_codec.codec.Decode.Trait T}
-        `{core.convert.From.Trait E (T := ErrorCode)}
-        `{core.ops.function.FnOnce.Trait F (Args := u32)}
-        `{core.ops.function.FnOnce.Trait D (Args := ref (Slice u8))}
+        `{H'0 : parity_scale_codec.codec.Encode.Trait I}
+        `{H'1 : parity_scale_codec.codec.Decode.Trait T}
+        `{H'2 : core.convert.From.Trait E (T := ErrorCode)}
+        `{H'3 : core.ops.function.FnOnce.Trait F (Args := u32)}
+        `{H'4 : core.ops.function.FnOnce.Trait D (Args := ref (Slice u8))}
         :=
-        call_chain_extension;
+        call_chain_extension
+            (I := I)
+            (T := T)
+            (E := E)
+            (ErrorCode := ErrorCode)
+            (F := F)
+            (D := D)
+          (H'0 := H'0)
+          (H'1 := H'1)
+          (H'2 := H'2)
+          (H'3 := H'3)
+          (H'4 := H'4);
     }.
     Global Instance Method_set_code_hash `{H' : State.Trait} `(Trait)
       : Notation.Dot "set_code_hash" := {
       Notation.dot := set_code_hash;
     }.
   End EnvBackend.
-End backend.
-
-Module contract.
-  Module ContractEnv.
-    Class Trait (Self : Set) : Type := {
-      Env : Set;
-      _ : exists `(ink_env.types.Environment.Trait Env), True;
-    }.
-    
-    Global Instance Method_Env `(Trait)
-      : Notation.DoubleColonType Self "Env" := {
-      Notation.double_colon_type := Env;
-    }.
-  End ContractEnv.
   
-  Module ContractReference.
-    Class Trait (Self : Set) : Type := {
-      Type_ : Set;
-    }.
-    
-    Global Instance Method_Type_ `(Trait)
-      : Notation.DoubleColonType Self "Type_" := {
-      Notation.double_colon_type := Type_;
-    }.
-  End ContractReference.
-End contract.
-
-Module call.
-  Module common.
-    Module ReturnType.
-      Section ReturnType.
-        Context {T : Set}.
-        Unset Primitive Projections.
-        Record t : Set := {
-          _ : core.marker.PhantomData (T);
-        }.
-        Global Set Primitive Projections.
-        
-        Global Instance Get_0 : Notation.Dot 0 := {
-          Notation.dot '(Build_t x0) := x0;
-        }.
-      End ReturnType.
-    End ReturnType.
-    Definition ReturnType := @ReturnType.t.
-    
-    Module Set_.
-      Section Set_.
-        Context {T : Set}.
-        Unset Primitive Projections.
-        Record t : Set := {
-          _ : T;
-        }.
-        Global Set Primitive Projections.
-        
-        Global Instance Get_0 : Notation.Dot 0 := {
-          Notation.dot '(Build_t x0) := x0;
-        }.
-      End Set_.
-    End Set_.
-    Definition Set_ := @Set_.t.
-    
-    Module Unset_.
-      Section Unset_.
-        Context {T : Set}.
-        Unset Primitive Projections.
-        Record t : Set := {
-          _ : core.marker.PhantomData (T);
-        }.
-        Global Set Primitive Projections.
-        
-        Global Instance Get_0 : Notation.Dot 0 := {
-          Notation.dot '(Build_t x0) := x0;
-        }.
-      End Unset_.
-    End Unset_.
-    Definition Unset_ := @Unset_.t.
-    
-    Module Unwrap.
-      Class Trait (Self : Set) : Type := {
-        Output : Set;
-        unwrap_or_else
-          `{H' : State.Trait}
-          {F: Set}
-          `{core.ops.function.FnOnce.Trait F (Args := unit)}
+  Module TypedEnvBackend.
+    Class Trait
+        (Self : Set)
+          `{ink_env.backend_and_call_builder_and_error.EnvBackend.Trait Self} :
+        Type := {
+      caller
+        `{H' : State.Trait}
+        {E: Set}
+        `{H'0 : ink_env.types.Environment.Trait E}
+        :
+        (mut_ref Self) -> (M (H := H') E::type["AccountId"]);
+      transferred_value
+        `{H' : State.Trait}
+        {E: Set}
+        `{H'0 : ink_env.types.Environment.Trait E}
+        :
+        (mut_ref Self) -> (M (H := H') E::type["Balance"]);
+      weight_to_fee
+        `{H' : State.Trait}
+        {E: Set}
+        `{H'0 : ink_env.types.Environment.Trait E}
+        :
+        (mut_ref Self) -> u64 -> (M (H := H') E::type["Balance"]);
+      gas_left
+        `{H' : State.Trait}
+        {E: Set}
+        `{H'0 : ink_env.types.Environment.Trait E}
+        :
+        (mut_ref Self) -> (M (H := H') u64);
+      block_timestamp
+        `{H' : State.Trait}
+        {E: Set}
+        `{H'0 : ink_env.types.Environment.Trait E}
+        :
+        (mut_ref Self) -> (M (H := H') E::type["Timestamp"]);
+      account_id
+        `{H' : State.Trait}
+        {E: Set}
+        `{H'0 : ink_env.types.Environment.Trait E}
+        :
+        (mut_ref Self) -> (M (H := H') E::type["AccountId"]);
+      balance
+        `{H' : State.Trait}
+        {E: Set}
+        `{H'0 : ink_env.types.Environment.Trait E}
+        :
+        (mut_ref Self) -> (M (H := H') E::type["Balance"]);
+      block_number
+        `{H' : State.Trait}
+        {E: Set}
+        `{H'0 : ink_env.types.Environment.Trait E}
+        :
+        (mut_ref Self) -> (M (H := H') E::type["BlockNumber"]);
+      minimum_balance
+        `{H' : State.Trait}
+        {E: Set}
+        `{H'0 : ink_env.types.Environment.Trait E}
+        :
+        (mut_ref Self) -> (M (H := H') E::type["Balance"]);
+      emit_event
+        `{H' : State.Trait}
+        {E Event: Set}
+        `{H'0 : ink_env.types.Environment.Trait E}
+        `{H'1 : ink_env.topics.Topics.Trait Event}
+        `{H'2 : parity_scale_codec.codec.Encode.Trait Event}
+        :
+        (mut_ref Self) -> Event -> (M (H := H') unit);
+      invoke_contract
+        `{H' : State.Trait}
+        {E Args R: Set}
+        `{H'0 : ink_env.types.Environment.Trait E}
+        `{H'1 : parity_scale_codec.codec.Encode.Trait Args}
+        `{H'2 : parity_scale_codec.codec.Decode.Trait R}
+        :
+        (mut_ref Self) ->
+        (ref
+          (ink_env.backend_and_call_builder_and_error.CallParams
+            E
+            (ink_env.backend_and_call_builder_and_error.Call E)
+            Args
+            R)) ->
+        (M (H := H')
+          (ink_env.backend_and_call_builder_and_error.Result
+            (ink_primitives.MessageResult R)));
+      invoke_contract_delegate
+        `{H' : State.Trait}
+        {E Args R: Set}
+        `{H'0 : ink_env.types.Environment.Trait E}
+        `{H'1 : parity_scale_codec.codec.Encode.Trait Args}
+        `{H'2 : parity_scale_codec.codec.Decode.Trait R}
+        :
+        (mut_ref Self) ->
+        (ref
+          (ink_env.backend_and_call_builder_and_error.CallParams
+            E
+            (ink_env.backend_and_call_builder_and_error.DelegateCall E)
+            Args
+            R)) ->
+        (M (H := H')
+          (ink_env.backend_and_call_builder_and_error.Result
+            (ink_primitives.MessageResult R)));
+      instantiate_contract
+        `{H' : State.Trait}
+        {E ContractRef Args Salt R: Set}
+        `{H'0 : ink_env.types.Environment.Trait E}
+        `{H'1
           :
-          Self -> F -> (M (H := H') Output);
-      }.
-      
-      Global Instance Method_Output `(Trait)
-        : Notation.DoubleColonType Self "Output" := {
-        Notation.double_colon_type := Output;
-      }.
-      Global Instance Method_unwrap_or_else `{H' : State.Trait} `(Trait)
-        : Notation.Dot "unwrap_or_else" := {
-        Notation.dot
-          {F : Set}
-          `{core.ops.function.FnOnce.Trait F (Args := unit)}
-          :=
-          unwrap_or_else;
-      }.
-    End Unwrap.
-  End common.
-  
-  Module selector.
-    Module Selector.
-      Unset Primitive Projections.
-      Record t : Set := {
-        bytes : list u8;
-      }.
-      Global Set Primitive Projections.
-      
-      Global Instance Get_bytes : Notation.Dot "bytes" := {
-        Notation.dot '(Build_t x0) := x0;
-      }.
-    End Selector.
-    Definition Selector : Set := Selector.t.
-  End selector.
-  
-  Module execution_input.
-    Module ExecutionInput.
-      Section ExecutionInput.
-        Context {Args : Set}.
-        Unset Primitive Projections.
-        Record t : Set := {
-          selector : ink_env.call.selector.Selector;
-          args : Args;
-        }.
-        Global Set Primitive Projections.
-        
-        Global Instance Get_selector : Notation.Dot "selector" := {
-          Notation.dot '(Build_t x0 _) := x0;
-        }.
-        Global Instance Get_args : Notation.Dot "args" := {
-          Notation.dot '(Build_t _ x1) := x1;
-        }.
-      End ExecutionInput.
-    End ExecutionInput.
-    Definition ExecutionInput (Args : Set) : Set :=
-      ExecutionInput.t (Args := Args).
-    
-    Module ArgumentList.
-      Section ArgumentList.
-        Context {Head Rest : Set}.
-        Unset Primitive Projections.
-        Record t : Set := {
-          head : Head;
-          rest : Rest;
-        }.
-        Global Set Primitive Projections.
-        
-        Global Instance Get_head : Notation.Dot "head" := {
-          Notation.dot '(Build_t x0 _) := x0;
-        }.
-        Global Instance Get_rest : Notation.Dot "rest" := {
-          Notation.dot '(Build_t _ x1) := x1;
-        }.
-      End ArgumentList.
-    End ArgumentList.
-    Definition ArgumentList (Head Rest : Set) : Set :=
-      ArgumentList.t (Head := Head) (Rest := Rest).
-    
-    Module Argument.
-      Section Argument.
-        Context {T : Set}.
-        Unset Primitive Projections.
-        Record t : Set := {
-          arg : T;
-        }.
-        Global Set Primitive Projections.
-        
-        Global Instance Get_arg : Notation.Dot "arg" := {
-          Notation.dot '(Build_t x0) := x0;
-        }.
-      End Argument.
-    End Argument.
-    Definition Argument (T : Set) : Set := Argument.t (T := T).
-    
-    Definition ArgsList (Head Rest : Set) : Set :=
-      ink_env.call.execution_input.ArgumentList
-        (ink_env.call.execution_input.Argument Head)
-        Rest.
-    
-    Module ArgumentListEnd.
-      Inductive t : Set := Build.
-    End ArgumentListEnd.
-    Definition ArgumentListEnd := @ArgumentListEnd.t.
-    
-    Definition EmptyArgumentList : Set :=
-      ink_env.call.execution_input.ArgumentList
-        ink_env.call.execution_input.ArgumentListEnd
-        ink_env.call.execution_input.ArgumentListEnd.
-  End execution_input.
-  
-  Module call_builder.
-    Module CallParams.
-      Section CallParams.
-        Context {E CallType Args R : Set}.
-        Context `{ink_env.types.Environment.Trait E}.
-        Unset Primitive Projections.
-        Record t : Set := {
-          call_type : CallType;
-          call_flags : ink_env.backend.CallFlags;
-          _return_type : ink_env.call.common.ReturnType R;
-          exec_input : ink_env.call.execution_input.ExecutionInput Args;
-          _phantom : core.marker.PhantomData (E);
-        }.
-        Global Set Primitive Projections.
-        
-        Global Instance Get_call_type : Notation.Dot "call_type" := {
-          Notation.dot '(Build_t x0 _ _ _ _) := x0;
-        }.
-        Global Instance Get_call_flags : Notation.Dot "call_flags" := {
-          Notation.dot '(Build_t _ x1 _ _ _) := x1;
-        }.
-        Global Instance Get__return_type : Notation.Dot "_return_type" := {
-          Notation.dot '(Build_t _ _ x2 _ _) := x2;
-        }.
-        Global Instance Get_exec_input : Notation.Dot "exec_input" := {
-          Notation.dot '(Build_t _ _ _ x3 _) := x3;
-        }.
-        Global Instance Get__phantom : Notation.Dot "_phantom" := {
-          Notation.dot '(Build_t _ _ _ _ x4) := x4;
-        }.
-      End CallParams.
-    End CallParams.
-    Definition CallParams
-        (E CallType Args R : Set)
-        `{ink_env.types.Environment.Trait E}
-        : Set :=
-      CallParams.t (E := E) (CallType := CallType) (Args := Args) (R := R).
-    
-    Module Call.
-      Section Call.
-        Context {E : Set}.
-        Context `{ink_env.types.Environment.Trait E}.
-        Unset Primitive Projections.
-        Record t : Set := {
-          callee : E::type["AccountId"];
-          gas_limit : ink_env.types.Gas;
-          transferred_value : E::type["Balance"];
-        }.
-        Global Set Primitive Projections.
-        
-        Global Instance Get_callee : Notation.Dot "callee" := {
-          Notation.dot '(Build_t x0 _ _) := x0;
-        }.
-        Global Instance Get_gas_limit : Notation.Dot "gas_limit" := {
-          Notation.dot '(Build_t _ x1 _) := x1;
-        }.
-        Global Instance Get_transferred_value
-          : Notation.Dot "transferred_value" := {
-          Notation.dot '(Build_t _ _ x2) := x2;
-        }.
-      End Call.
-    End Call.
-    Definition Call (E : Set) `{ink_env.types.Environment.Trait E} : Set :=
-      Call.t (E := E).
-    
-    Module CallBuilder.
-      Section CallBuilder.
-        Context {E CallType Args RetType : Set}.
-        Context `{ink_env.types.Environment.Trait E}.
-        Unset Primitive Projections.
-        Record t : Set := {
-          call_type : CallType;
-          call_flags : ink_env.backend.CallFlags;
-          exec_input : Args;
-          return_type : RetType;
-          _phantom : core.marker.PhantomData (E);
-        }.
-        Global Set Primitive Projections.
-        
-        Global Instance Get_call_type : Notation.Dot "call_type" := {
-          Notation.dot '(Build_t x0 _ _ _ _) := x0;
-        }.
-        Global Instance Get_call_flags : Notation.Dot "call_flags" := {
-          Notation.dot '(Build_t _ x1 _ _ _) := x1;
-        }.
-        Global Instance Get_exec_input : Notation.Dot "exec_input" := {
-          Notation.dot '(Build_t _ _ x2 _ _) := x2;
-        }.
-        Global Instance Get_return_type : Notation.Dot "return_type" := {
-          Notation.dot '(Build_t _ _ _ x3 _) := x3;
-        }.
-        Global Instance Get__phantom : Notation.Dot "_phantom" := {
-          Notation.dot '(Build_t _ _ _ _ x4) := x4;
-        }.
-      End CallBuilder.
-    End CallBuilder.
-    Definition CallBuilder
-        (E CallType Args RetType : Set)
-        `{ink_env.types.Environment.Trait E}
-        : Set :=
-      CallBuilder.t
-        (E := E)
-        (CallType := CallType)
-        (Args := Args)
-        (RetType := RetType).
-    
-    Parameter build_call :
-        forall
-          `{H' : State.Trait}
-          {E : Set}
-          `{ink_env.types.Environment.Trait E},
-        M (H := H')
-            (ink_env.call.call_builder.CallBuilder
-              E
-              (ink_env.call.common.Unset_ (ink_env.call.call_builder.Call E))
-              (ink_env.call.common.Unset_
-                (ink_env.call.execution_input.ExecutionInput
-                  ink_env.call.execution_input.EmptyArgumentList))
-              (ink_env.call.common.Unset_
-                (ink_env.call.common.ReturnType unit))).
-    
-    Module DelegateCall.
-      Section DelegateCall.
-        Context {E : Set}.
-        Context `{ink_env.types.Environment.Trait E}.
-        Unset Primitive Projections.
-        Record t : Set := {
-          code_hash : E::type["Hash"];
-        }.
-        Global Set Primitive Projections.
-        
-        Global Instance Get_code_hash : Notation.Dot "code_hash" := {
-          Notation.dot '(Build_t x0) := x0;
-        }.
-      End DelegateCall.
-    End DelegateCall.
-    Definition DelegateCall
-        (E : Set)
-        `{ink_env.types.Environment.Trait E}
-        : Set :=
-      DelegateCall.t (E := E).
-  End call_builder.
-  
-  Module create_builder.
-    Module state.
-      Module Salt.
-        Inductive t : Set :=
-        .
-      End Salt.
-      Definition Salt := Salt.t.
-    End state.
-    
-    Module FromAccountId.
-      Class Trait
-          (Self : Set) {T : Set} `{ink_env.types.Environment.Trait T} :
-          Type := {
-        from_account_id
-          `{H' : State.Trait}
+          ink_env.call.create_builder.FromAccountId.Trait ContractRef (T := E)}
+        `{H'2 : parity_scale_codec.codec.Encode.Trait Args}
+        `{H'3 : core.convert.AsRef.Trait Salt (T := Slice u8)}
+        `{H'4
           :
-          ink_env.types.Environment.AccountId -> (M (H := H') Self);
-      }.
-      
-      Global Instance Method_from_account_id `{H' : State.Trait} `(Trait)
-        : Notation.Dot "from_account_id" := {
-        Notation.dot := from_account_id;
-      }.
-    End FromAccountId.
+          ink_env.call.create_builder.ConstructorReturnType.Trait R
+            (C := ContractRef)}
+        :
+        (mut_ref Self) ->
+        (ref
+          (ink_env.call.create_builder.CreateParams
+            E
+            ContractRef
+            Args
+            Salt
+            R)) ->
+        (M (H := H')
+          (ink_env.backend_and_call_builder_and_error.Result
+            (ink_primitives.ConstructorResult
+              ink_env.call.create_builder.ConstructorReturnType.Output)));
+      terminate_contract
+        `{H' : State.Trait}
+        {E: Set}
+        `{H'0 : ink_env.types.Environment.Trait E}
+        :
+        (mut_ref Self) -> E::type["AccountId"] -> (M (H := H') Empty_set);
+      transfer
+        `{H' : State.Trait}
+        {E: Set}
+        `{H'0 : ink_env.types.Environment.Trait E}
+        :
+        (mut_ref Self) ->
+        E::type["AccountId"] ->
+        E::type["Balance"] ->
+        (M (H := H') (ink_env.backend_and_call_builder_and_error.Result unit));
+      is_contract
+        `{H' : State.Trait}
+        {E: Set}
+        `{H'0 : ink_env.types.Environment.Trait E}
+        :
+        (mut_ref Self) -> (ref E::type["AccountId"]) -> (M (H := H') bool);
+      caller_is_origin
+        `{H' : State.Trait}
+        {E: Set}
+        `{H'0 : ink_env.types.Environment.Trait E}
+        :
+        (mut_ref Self) -> (M (H := H') bool);
+      code_hash
+        `{H' : State.Trait}
+        {E: Set}
+        `{H'0 : ink_env.types.Environment.Trait E}
+        :
+        (mut_ref Self) ->
+        (ref E::type["AccountId"]) ->
+        (M (H := H')
+          (ink_env.backend_and_call_builder_and_error.Result E::type["Hash"]));
+      own_code_hash
+        `{H' : State.Trait}
+        {E: Set}
+        `{H'0 : ink_env.types.Environment.Trait E}
+        :
+        (mut_ref Self) ->
+        (M (H := H')
+          (ink_env.backend_and_call_builder_and_error.Result E::type["Hash"]));
+      call_runtime
+        `{H' : State.Trait}
+        {E Call: Set}
+        `{H'0 : ink_env.types.Environment.Trait E}
+        `{H'1 : parity_scale_codec.codec.Encode.Trait Call}
+        :
+        (mut_ref Self) ->
+        (ref Call) ->
+        (M (H := H') (ink_env.backend_and_call_builder_and_error.Result unit));
+    }.
     
-    Module ConstructorReturnType.
-      Class Trait (Self : Set) {C : Set} : Type := {
-        IS_RESULT `{H' : State.Trait} : bool;
-        Output : Set;
-        Error : Set;
-        _ : exists `(parity_scale_codec.codec.Decode.Trait Error), True;
-        ok `{H' : State.Trait} : C -> (M (H := H') Output);
-      }.
-      
-      Global Instance Method_IS_RESULT `{H' : State.Trait} `(Trait)
-        : Notation.Dot "IS_RESULT" := {
-        Notation.dot := IS_RESULT;
-      }.
-      Global Instance Method_Output `(Trait)
-        : Notation.DoubleColonType Self "Output" := {
-        Notation.double_colon_type := Output;
-      }.
-      Global Instance Method_Error `(Trait)
-        : Notation.DoubleColonType Self "Error" := {
-        Notation.double_colon_type := Error;
-      }.
-      Global Instance Method_ok `{H' : State.Trait} `(Trait)
-        : Notation.Dot "ok" := {
-        Notation.dot := ok;
-      }.
-      Global Instance Method_err `{H' : State.Trait} `(Trait)
-        : Notation.Dot "err" := {
-        Notation.dot (_err : Error)
-          :=
-          (axiom : M (H := H') (core.option.Option Output));
-      }.
-    End ConstructorReturnType.
-    
-    Module CreateParams.
-      Section CreateParams.
-        Context {E ContractRef Args Salt R : Set}.
-        Context `{ink_env.types.Environment.Trait E}.
-        Unset Primitive Projections.
-        Record t : Set := {
-          code_hash : E::type["Hash"];
-          gas_limit : u64;
-          endowment : E::type["Balance"];
-          exec_input : ink_env.call.execution_input.ExecutionInput Args;
-          salt_bytes : Salt;
-          _return_type : ink_env.call.common.ReturnType R;
-          _phantom : core.marker.PhantomData (ContractRef);
-        }.
-        Global Set Primitive Projections.
-        
-        Global Instance Get_code_hash : Notation.Dot "code_hash" := {
-          Notation.dot '(Build_t x0 _ _ _ _ _ _) := x0;
-        }.
-        Global Instance Get_gas_limit : Notation.Dot "gas_limit" := {
-          Notation.dot '(Build_t _ x1 _ _ _ _ _) := x1;
-        }.
-        Global Instance Get_endowment : Notation.Dot "endowment" := {
-          Notation.dot '(Build_t _ _ x2 _ _ _ _) := x2;
-        }.
-        Global Instance Get_exec_input : Notation.Dot "exec_input" := {
-          Notation.dot '(Build_t _ _ _ x3 _ _ _) := x3;
-        }.
-        Global Instance Get_salt_bytes : Notation.Dot "salt_bytes" := {
-          Notation.dot '(Build_t _ _ _ _ x4 _ _) := x4;
-        }.
-        Global Instance Get__return_type : Notation.Dot "_return_type" := {
-          Notation.dot '(Build_t _ _ _ _ _ x5 _) := x5;
-        }.
-        Global Instance Get__phantom : Notation.Dot "_phantom" := {
-          Notation.dot '(Build_t _ _ _ _ _ _ x6) := x6;
-        }.
-      End CreateParams.
-    End CreateParams.
-    Definition CreateParams
-        (E ContractRef Args Salt R : Set)
-        `{ink_env.types.Environment.Trait E}
-        : Set :=
-      CreateParams.t
-        (E := E)
-        (ContractRef := ContractRef)
-        (Args := Args)
-        (Salt := Salt)
-        (R := R).
-    
-    Module CreateBuilder.
-      Section CreateBuilder.
-        Context
-          {E ContractRef CodeHash GasLimit Endowment Args Salt RetType : Set}.
-        Context `{ink_env.types.Environment.Trait E}.
-        Unset Primitive Projections.
-        Record t : Set := {
-          code_hash : CodeHash;
-          gas_limit : GasLimit;
-          endowment : Endowment;
-          exec_input : Args;
-          salt : Salt;
-          return_type : RetType;
-          _phantom : core.marker.PhantomData (E * ContractRef);
-        }.
-        Global Set Primitive Projections.
-        
-        Global Instance Get_code_hash : Notation.Dot "code_hash" := {
-          Notation.dot '(Build_t x0 _ _ _ _ _ _) := x0;
-        }.
-        Global Instance Get_gas_limit : Notation.Dot "gas_limit" := {
-          Notation.dot '(Build_t _ x1 _ _ _ _ _) := x1;
-        }.
-        Global Instance Get_endowment : Notation.Dot "endowment" := {
-          Notation.dot '(Build_t _ _ x2 _ _ _ _) := x2;
-        }.
-        Global Instance Get_exec_input : Notation.Dot "exec_input" := {
-          Notation.dot '(Build_t _ _ _ x3 _ _ _) := x3;
-        }.
-        Global Instance Get_salt : Notation.Dot "salt" := {
-          Notation.dot '(Build_t _ _ _ _ x4 _ _) := x4;
-        }.
-        Global Instance Get_return_type : Notation.Dot "return_type" := {
-          Notation.dot '(Build_t _ _ _ _ _ x5 _) := x5;
-        }.
-        Global Instance Get__phantom : Notation.Dot "_phantom" := {
-          Notation.dot '(Build_t _ _ _ _ _ _ x6) := x6;
-        }.
-      End CreateBuilder.
-    End CreateBuilder.
-    Definition CreateBuilder
-        (E ContractRef CodeHash GasLimit Endowment Args Salt RetType : Set)
-        `{ink_env.types.Environment.Trait E}
-        : Set :=
-      CreateBuilder.t
-        (E := E)
-        (ContractRef := ContractRef)
-        (CodeHash := CodeHash)
-        (GasLimit := GasLimit)
-        (Endowment := Endowment)
-        (Args := Args)
-        (Salt := Salt)
-        (RetType := RetType).
-  End create_builder.
-End call.
+    Global Instance Method_caller `{H' : State.Trait} `(Trait)
+      : Notation.Dot "caller" := {
+      Notation.dot {E : Set} `{H'0 : ink_env.types.Environment.Trait E}
+        :=
+        caller (E := E) (H'0 := H'0);
+    }.
+    Global Instance Method_transferred_value `{H' : State.Trait} `(Trait)
+      : Notation.Dot "transferred_value" := {
+      Notation.dot {E : Set} `{H'0 : ink_env.types.Environment.Trait E}
+        :=
+        transferred_value (E := E) (H'0 := H'0);
+    }.
+    Global Instance Method_weight_to_fee `{H' : State.Trait} `(Trait)
+      : Notation.Dot "weight_to_fee" := {
+      Notation.dot {E : Set} `{H'0 : ink_env.types.Environment.Trait E}
+        :=
+        weight_to_fee (E := E) (H'0 := H'0);
+    }.
+    Global Instance Method_gas_left `{H' : State.Trait} `(Trait)
+      : Notation.Dot "gas_left" := {
+      Notation.dot {E : Set} `{H'0 : ink_env.types.Environment.Trait E}
+        :=
+        gas_left (E := E) (H'0 := H'0);
+    }.
+    Global Instance Method_block_timestamp `{H' : State.Trait} `(Trait)
+      : Notation.Dot "block_timestamp" := {
+      Notation.dot {E : Set} `{H'0 : ink_env.types.Environment.Trait E}
+        :=
+        block_timestamp (E := E) (H'0 := H'0);
+    }.
+    Global Instance Method_account_id `{H' : State.Trait} `(Trait)
+      : Notation.Dot "account_id" := {
+      Notation.dot {E : Set} `{H'0 : ink_env.types.Environment.Trait E}
+        :=
+        account_id (E := E) (H'0 := H'0);
+    }.
+    Global Instance Method_balance `{H' : State.Trait} `(Trait)
+      : Notation.Dot "balance" := {
+      Notation.dot {E : Set} `{H'0 : ink_env.types.Environment.Trait E}
+        :=
+        balance (E := E) (H'0 := H'0);
+    }.
+    Global Instance Method_block_number `{H' : State.Trait} `(Trait)
+      : Notation.Dot "block_number" := {
+      Notation.dot {E : Set} `{H'0 : ink_env.types.Environment.Trait E}
+        :=
+        block_number (E := E) (H'0 := H'0);
+    }.
+    Global Instance Method_minimum_balance `{H' : State.Trait} `(Trait)
+      : Notation.Dot "minimum_balance" := {
+      Notation.dot {E : Set} `{H'0 : ink_env.types.Environment.Trait E}
+        :=
+        minimum_balance (E := E) (H'0 := H'0);
+    }.
+    Global Instance Method_emit_event `{H' : State.Trait} `(Trait)
+      : Notation.Dot "emit_event" := {
+      Notation.dot
+        {E Event : Set}
+        `{H'0 : ink_env.types.Environment.Trait E}
+        `{H'1 : ink_env.topics.Topics.Trait Event}
+        `{H'2 : parity_scale_codec.codec.Encode.Trait Event}
+        :=
+        emit_event (E := E) (Event := Event)
+          (H'0 := H'0)
+          (H'1 := H'1)
+          (H'2 := H'2);
+    }.
+    Global Instance Method_invoke_contract `{H' : State.Trait} `(Trait)
+      : Notation.Dot "invoke_contract" := {
+      Notation.dot
+        {E Args R : Set}
+        `{H'0 : ink_env.types.Environment.Trait E}
+        `{H'1 : parity_scale_codec.codec.Encode.Trait Args}
+        `{H'2 : parity_scale_codec.codec.Decode.Trait R}
+        :=
+        invoke_contract (E := E) (Args := Args) (R := R)
+          (H'0 := H'0)
+          (H'1 := H'1)
+          (H'2 := H'2);
+    }.
+    Global Instance Method_invoke_contract_delegate `{H' : State.Trait} `(Trait)
+      : Notation.Dot "invoke_contract_delegate" := {
+      Notation.dot
+        {E Args R : Set}
+        `{H'0 : ink_env.types.Environment.Trait E}
+        `{H'1 : parity_scale_codec.codec.Encode.Trait Args}
+        `{H'2 : parity_scale_codec.codec.Decode.Trait R}
+        :=
+        invoke_contract_delegate (E := E) (Args := Args) (R := R)
+          (H'0 := H'0)
+          (H'1 := H'1)
+          (H'2 := H'2);
+    }.
+    Global Instance Method_instantiate_contract `{H' : State.Trait} `(Trait)
+      : Notation.Dot "instantiate_contract" := {
+      Notation.dot
+        {E ContractRef Args Salt R : Set}
+        `{H'0 : ink_env.types.Environment.Trait E}
+        `{H'1
+          :
+          ink_env.call.create_builder.FromAccountId.Trait ContractRef (T := E)}
+        `{H'2 : parity_scale_codec.codec.Encode.Trait Args}
+        `{H'3 : core.convert.AsRef.Trait Salt (T := Slice u8)}
+        `{H'4
+          :
+          ink_env.call.create_builder.ConstructorReturnType.Trait R
+            (C := ContractRef)}
+        :=
+        instantiate_contract
+            (E := E)
+            (ContractRef := ContractRef)
+            (Args := Args)
+            (Salt := Salt)
+            (R := R)
+          (H'0 := H'0)
+          (H'1 := H'1)
+          (H'2 := H'2)
+          (H'3 := H'3)
+          (H'4 := H'4);
+    }.
+    Global Instance Method_terminate_contract `{H' : State.Trait} `(Trait)
+      : Notation.Dot "terminate_contract" := {
+      Notation.dot {E : Set} `{H'0 : ink_env.types.Environment.Trait E}
+        :=
+        terminate_contract (E := E) (H'0 := H'0);
+    }.
+    Global Instance Method_transfer `{H' : State.Trait} `(Trait)
+      : Notation.Dot "transfer" := {
+      Notation.dot {E : Set} `{H'0 : ink_env.types.Environment.Trait E}
+        :=
+        transfer (E := E) (H'0 := H'0);
+    }.
+    Global Instance Method_is_contract `{H' : State.Trait} `(Trait)
+      : Notation.Dot "is_contract" := {
+      Notation.dot {E : Set} `{H'0 : ink_env.types.Environment.Trait E}
+        :=
+        is_contract (E := E) (H'0 := H'0);
+    }.
+    Global Instance Method_caller_is_origin `{H' : State.Trait} `(Trait)
+      : Notation.Dot "caller_is_origin" := {
+      Notation.dot {E : Set} `{H'0 : ink_env.types.Environment.Trait E}
+        :=
+        caller_is_origin (E := E) (H'0 := H'0);
+    }.
+    Global Instance Method_code_hash `{H' : State.Trait} `(Trait)
+      : Notation.Dot "code_hash" := {
+      Notation.dot {E : Set} `{H'0 : ink_env.types.Environment.Trait E}
+        :=
+        code_hash (E := E) (H'0 := H'0);
+    }.
+    Global Instance Method_own_code_hash `{H' : State.Trait} `(Trait)
+      : Notation.Dot "own_code_hash" := {
+      Notation.dot {E : Set} `{H'0 : ink_env.types.Environment.Trait E}
+        :=
+        own_code_hash (E := E) (H'0 := H'0);
+    }.
+    Global Instance Method_call_runtime `{H' : State.Trait} `(Trait)
+      : Notation.Dot "call_runtime" := {
+      Notation.dot
+        {E Call : Set}
+        `{H'0 : ink_env.types.Environment.Trait E}
+        `{H'1 : parity_scale_codec.codec.Encode.Trait Call}
+        :=
+        call_runtime (E := E) (Call := Call) (H'0 := H'0) (H'1 := H'1);
+    }.
+  End TypedEnvBackend.
+End backend_and_call_builder_and_error.
 
 Module api.
   Parameter caller :
@@ -1707,7 +2068,10 @@ Module api.
         {K R : Set}
         `{parity_scale_codec.codec.Encode.Trait K}
         `{ink_storage_traits.storage.Storable.Trait R},
-      (ref K) -> M (H := H') (ink_env.error.Result (core.option.Option R)).
+      (ref K) ->
+        M (H := H')
+          (ink_env.backend_and_call_builder_and_error.Result
+            (core.option.Option R)).
   
   Parameter take_contract_storage :
       forall
@@ -1715,7 +2079,10 @@ Module api.
         {K R : Set}
         `{parity_scale_codec.codec.Encode.Trait K}
         `{ink_storage_traits.storage.Storable.Trait R},
-      (ref K) -> M (H := H') (ink_env.error.Result (core.option.Option R)).
+      (ref K) ->
+        M (H := H')
+          (ink_env.backend_and_call_builder_and_error.Result
+            (core.option.Option R)).
   
   Parameter contains_contract_storage :
       forall
@@ -1739,13 +2106,15 @@ Module api.
         `{parity_scale_codec.codec.Encode.Trait Args}
         `{parity_scale_codec.codec.Decode.Trait R},
       (ref
-          (ink_env.call.call_builder.CallParams
+          (ink_env.backend_and_call_builder_and_error.CallParams
             E
-            (ink_env.call.call_builder.Call E)
+            (ink_env.backend_and_call_builder_and_error.Call E)
             Args
             R))
         ->
-        M (H := H') (ink_env.error.Result (ink_primitives.MessageResult R)).
+        M (H := H')
+          (ink_env.backend_and_call_builder_and_error.Result
+            (ink_primitives.MessageResult R)).
   
   Parameter invoke_contract_delegate :
       forall
@@ -1755,13 +2124,15 @@ Module api.
         `{parity_scale_codec.codec.Encode.Trait Args}
         `{parity_scale_codec.codec.Decode.Trait R},
       (ref
-          (ink_env.call.call_builder.CallParams
+          (ink_env.backend_and_call_builder_and_error.CallParams
             E
-            (ink_env.call.call_builder.DelegateCall E)
+            (ink_env.backend_and_call_builder_and_error.DelegateCall E)
             Args
             R))
         ->
-        M (H := H') (ink_env.error.Result (ink_primitives.MessageResult R)).
+        M (H := H')
+          (ink_env.backend_and_call_builder_and_error.Result
+            (ink_primitives.MessageResult R)).
   
   Parameter instantiate_contract :
       forall
@@ -1776,7 +2147,7 @@ Module api.
       (ref (ink_env.call.create_builder.CreateParams E ContractRef Args Salt R))
         ->
         M (H := H')
-          (ink_env.error.Result
+          (ink_env.backend_and_call_builder_and_error.Result
             (ink_primitives.ConstructorResult
               ink_env.call.create_builder.ConstructorReturnType.Output)).
   
@@ -1788,21 +2159,23 @@ Module api.
       forall `{H' : State.Trait} {E : Set} `{ink_env.types.Environment.Trait E},
       E::type["AccountId"] ->
         E::type["Balance"] ->
-        M (H := H') (ink_env.error.Result unit).
+        M (H := H') (ink_env.backend_and_call_builder_and_error.Result unit).
   
   Parameter decode_input :
       forall
         `{H' : State.Trait}
         {T : Set}
         `{parity_scale_codec.codec.Decode.Trait T},
-      M (H := H') (ink_env.error.Result T).
+      M (H := H') (ink_env.backend_and_call_builder_and_error.Result T).
   
   Parameter return_value :
       forall
         `{H' : State.Trait}
         {R : Set}
         `{parity_scale_codec.codec.Encode.Trait R},
-      ink_env.backend.ReturnFlags -> (ref R) -> M (H := H') Empty_set.
+      ink_env.backend_and_call_builder_and_error.ReturnFlags ->
+        (ref R) ->
+        M (H := H') Empty_set.
   
   Parameter debug_message :
       forall `{H' : State.Trait},
@@ -1827,13 +2200,13 @@ Module api.
       (ref (list u8)) ->
         (ref (list u8)) ->
         (mut_ref (list u8)) ->
-        M (H := H') (ink_env.error.Result unit).
+        M (H := H') (ink_env.backend_and_call_builder_and_error.Result unit).
   
   Parameter ecdsa_to_eth_address :
       forall `{H' : State.Trait},
       (ref (list u8)) ->
         (mut_ref (list u8)) ->
-        M (H := H') (ink_env.error.Result unit).
+        M (H := H') (ink_env.backend_and_call_builder_and_error.Result unit).
   
   Parameter is_contract :
       forall `{H' : State.Trait} {E : Set} `{ink_env.types.Environment.Trait E},
@@ -1842,11 +2215,13 @@ Module api.
   Parameter code_hash :
       forall `{H' : State.Trait} {E : Set} `{ink_env.types.Environment.Trait E},
       (ref E::type["AccountId"]) ->
-        M (H := H') (ink_env.error.Result E::type["Hash"]).
+        M (H := H')
+          (ink_env.backend_and_call_builder_and_error.Result E::type["Hash"]).
   
   Parameter own_code_hash :
       forall `{H' : State.Trait} {E : Set} `{ink_env.types.Environment.Trait E},
-      M (H := H') (ink_env.error.Result E::type["Hash"]).
+      M (H := H')
+          (ink_env.backend_and_call_builder_and_error.Result E::type["Hash"]).
   
   Parameter caller_is_origin :
       forall `{H' : State.Trait} {E : Set} `{ink_env.types.Environment.Trait E},
@@ -1854,11 +2229,13 @@ Module api.
   
   Parameter set_code_hash :
       forall `{H' : State.Trait},
-      (ref (list u8)) -> M (H := H') (ink_env.error.Result unit).
+      (ref (list u8)) ->
+        M (H := H') (ink_env.backend_and_call_builder_and_error.Result unit).
   
   Parameter set_code_hash2 :
       forall `{H' : State.Trait} {E : Set} `{ink_env.types.Environment.Trait E},
-      (ref E::type["Hash"]) -> M (H := H') (ink_env.error.Result unit).
+      (ref E::type["Hash"]) ->
+        M (H := H') (ink_env.backend_and_call_builder_and_error.Result unit).
   
   Parameter call_runtime :
       forall
@@ -1866,7 +2243,8 @@ Module api.
         {E Call : Set}
         `{ink_env.types.Environment.Trait E}
         `{parity_scale_codec.codec.Encode.Trait Call},
-      (ref Call) -> M (H := H') (ink_env.error.Result unit).
+      (ref Call) ->
+        M (H := H') (ink_env.backend_and_call_builder_and_error.Result unit).
 End api.
 
 Parameter caller :
@@ -1928,7 +2306,10 @@ Parameter get_contract_storage :
       {K R : Set}
       `{parity_scale_codec.codec.Encode.Trait K}
       `{ink_storage_traits.storage.Storable.Trait R},
-    (ref K) -> M (H := H') (ink_env.error.Result (core.option.Option R)).
+    (ref K) ->
+      M (H := H')
+        (ink_env.backend_and_call_builder_and_error.Result
+          (core.option.Option R)).
 
 Parameter take_contract_storage :
     forall
@@ -1936,7 +2317,10 @@ Parameter take_contract_storage :
       {K R : Set}
       `{parity_scale_codec.codec.Encode.Trait K}
       `{ink_storage_traits.storage.Storable.Trait R},
-    (ref K) -> M (H := H') (ink_env.error.Result (core.option.Option R)).
+    (ref K) ->
+      M (H := H')
+        (ink_env.backend_and_call_builder_and_error.Result
+          (core.option.Option R)).
 
 Parameter contains_contract_storage :
     forall
@@ -1952,11 +2336,58 @@ Parameter clear_contract_storage :
       `{parity_scale_codec.codec.Encode.Trait K},
     (ref K) -> M (H := H') (core.option.Option u32).
 
+Parameter invoke_contract :
+    forall
+      `{H' : State.Trait}
+      {E Args R : Set}
+      `{ink_env.types.Environment.Trait E}
+      `{parity_scale_codec.codec.Encode.Trait Args}
+      `{parity_scale_codec.codec.Decode.Trait R},
+    (ref
+        (ink_env.backend_and_call_builder_and_error.CallParams
+          E
+          (ink_env.backend_and_call_builder_and_error.Call E)
+          Args
+          R))
+      ->
+      M (H := H')
+        (ink_env.backend_and_call_builder_and_error.Result
+          (ink_primitives.MessageResult R)).
 
+Parameter invoke_contract_delegate :
+    forall
+      `{H' : State.Trait}
+      {E Args R : Set}
+      `{ink_env.types.Environment.Trait E}
+      `{parity_scale_codec.codec.Encode.Trait Args}
+      `{parity_scale_codec.codec.Decode.Trait R},
+    (ref
+        (ink_env.backend_and_call_builder_and_error.CallParams
+          E
+          (ink_env.backend_and_call_builder_and_error.DelegateCall E)
+          Args
+          R))
+      ->
+      M (H := H')
+        (ink_env.backend_and_call_builder_and_error.Result
+          (ink_primitives.MessageResult R)).
 
-
-
-
+Parameter instantiate_contract :
+    forall
+      `{H' : State.Trait}
+      {E ContractRef Args Salt R : Set}
+      `{ink_env.types.Environment.Trait E}
+      `{ink_env.call.create_builder.FromAccountId.Trait ContractRef (T := E)}
+      `{parity_scale_codec.codec.Encode.Trait Args}
+      `{core.convert.AsRef.Trait Salt (T := Slice u8)}
+      `{ink_env.call.create_builder.ConstructorReturnType.Trait R
+          (C := ContractRef)},
+    (ref (ink_env.call.create_builder.CreateParams E ContractRef Args Salt R))
+      ->
+      M (H := H')
+        (ink_env.backend_and_call_builder_and_error.Result
+          (ink_primitives.ConstructorResult
+            ink_env.call.create_builder.ConstructorReturnType.Output)).
 
 Parameter terminate_contract :
     forall `{H' : State.Trait} {E : Set} `{ink_env.types.Environment.Trait E},
@@ -1966,21 +2397,23 @@ Parameter transfer :
     forall `{H' : State.Trait} {E : Set} `{ink_env.types.Environment.Trait E},
     E::type["AccountId"] ->
       E::type["Balance"] ->
-      M (H := H') (ink_env.error.Result unit).
+      M (H := H') (ink_env.backend_and_call_builder_and_error.Result unit).
 
 Parameter decode_input :
     forall
       `{H' : State.Trait}
       {T : Set}
       `{parity_scale_codec.codec.Decode.Trait T},
-    M (H := H') (ink_env.error.Result T).
+    M (H := H') (ink_env.backend_and_call_builder_and_error.Result T).
 
 Parameter return_value :
     forall
       `{H' : State.Trait}
       {R : Set}
       `{parity_scale_codec.codec.Encode.Trait R},
-    ink_env.backend.ReturnFlags -> (ref R) -> M (H := H') Empty_set.
+    ink_env.backend_and_call_builder_and_error.ReturnFlags ->
+      (ref R) ->
+      M (H := H') Empty_set.
 
 Parameter debug_message :
     forall `{H' : State.Trait},
@@ -2005,13 +2438,13 @@ Parameter ecdsa_recover :
     (ref (list u8)) ->
       (ref (list u8)) ->
       (mut_ref (list u8)) ->
-      M (H := H') (ink_env.error.Result unit).
+      M (H := H') (ink_env.backend_and_call_builder_and_error.Result unit).
 
 Parameter ecdsa_to_eth_address :
     forall `{H' : State.Trait},
     (ref (list u8)) ->
       (mut_ref (list u8)) ->
-      M (H := H') (ink_env.error.Result unit).
+      M (H := H') (ink_env.backend_and_call_builder_and_error.Result unit).
 
 Parameter is_contract :
     forall `{H' : State.Trait} {E : Set} `{ink_env.types.Environment.Trait E},
@@ -2020,11 +2453,13 @@ Parameter is_contract :
 Parameter code_hash :
     forall `{H' : State.Trait} {E : Set} `{ink_env.types.Environment.Trait E},
     (ref E::type["AccountId"]) ->
-      M (H := H') (ink_env.error.Result E::type["Hash"]).
+      M (H := H')
+        (ink_env.backend_and_call_builder_and_error.Result E::type["Hash"]).
 
 Parameter own_code_hash :
     forall `{H' : State.Trait} {E : Set} `{ink_env.types.Environment.Trait E},
-    M (H := H') (ink_env.error.Result E::type["Hash"]).
+    M (H := H')
+        (ink_env.backend_and_call_builder_and_error.Result E::type["Hash"]).
 
 Parameter caller_is_origin :
     forall `{H' : State.Trait} {E : Set} `{ink_env.types.Environment.Trait E},
@@ -2032,11 +2467,13 @@ Parameter caller_is_origin :
 
 Parameter set_code_hash :
     forall `{H' : State.Trait},
-    (ref (list u8)) -> M (H := H') (ink_env.error.Result unit).
+    (ref (list u8)) ->
+      M (H := H') (ink_env.backend_and_call_builder_and_error.Result unit).
 
 Parameter set_code_hash2 :
     forall `{H' : State.Trait} {E : Set} `{ink_env.types.Environment.Trait E},
-    (ref E::type["Hash"]) -> M (H := H') (ink_env.error.Result unit).
+    (ref E::type["Hash"]) ->
+      M (H := H') (ink_env.backend_and_call_builder_and_error.Result unit).
 
 Parameter call_runtime :
     forall
@@ -2044,7 +2481,8 @@ Parameter call_runtime :
       {E Call : Set}
       `{ink_env.types.Environment.Trait E}
       `{parity_scale_codec.codec.Encode.Trait Call},
-    (ref Call) -> M (H := H') (ink_env.error.Result unit).
+    (ref Call) ->
+      M (H := H') (ink_env.backend_and_call_builder_and_error.Result unit).
 
 Module BaseArithmetic.
   Unset Primitive Projections.
@@ -2132,396 +2570,27 @@ Module Saturating.
   }.
 End Saturating.
 
-Module ReturnFlags.
-  Unset Primitive Projections.
-  Record t : Set := {
-    value : u32;
-  }.
-  Global Set Primitive Projections.
-  
-  Global Instance Get_value : Notation.Dot "value" := {
-    Notation.dot '(Build_t x0) := x0;
-  }.
-End ReturnFlags.
-Definition ReturnFlags : Set := ReturnFlags.t.
+Module Error.
+  Inductive t : Set :=
+  | Decode (_ : parity_scale_codec.error.Error)
+  | OffChain (_ : ink_env.engine.off_chain.OffChainError)
+  | CalleeTrapped
+  | CalleeReverted
+  | KeyNotFound
+  | _BelowSubsistenceThreshold
+  | TransferFailed
+  | _EndowmentTooLow
+  | CodeNotFound
+  | NotCallable
+  | Unknown
+  | LoggingDisabled
+  | CallRuntimeFailed
+  | EcdsaRecoveryFailed.
+End Error.
+Definition Error := Error.t.
 
-Module CallFlags.
-  Unset Primitive Projections.
-  Record t : Set := {
-    forward_input : bool;
-    clone_input : bool;
-    tail_call : bool;
-    allow_reentry : bool;
-  }.
-  Global Set Primitive Projections.
-  
-  Global Instance Get_forward_input : Notation.Dot "forward_input" := {
-    Notation.dot '(Build_t x0 _ _ _) := x0;
-  }.
-  Global Instance Get_clone_input : Notation.Dot "clone_input" := {
-    Notation.dot '(Build_t _ x1 _ _) := x1;
-  }.
-  Global Instance Get_tail_call : Notation.Dot "tail_call" := {
-    Notation.dot '(Build_t _ _ x2 _) := x2;
-  }.
-  Global Instance Get_allow_reentry : Notation.Dot "allow_reentry" := {
-    Notation.dot '(Build_t _ _ _ x3) := x3;
-  }.
-End CallFlags.
-Definition CallFlags : Set := CallFlags.t.
-
-Module EnvBackend.
-  Class Trait (Self : Set) : Type := {
-    set_contract_storage
-      `{H' : State.Trait}
-      {K V: Set}
-      `{parity_scale_codec.codec.Encode.Trait K}
-      `{ink_storage_traits.storage.Storable.Trait V}
-      :
-      (mut_ref Self) ->
-      (ref K) ->
-      (ref V) ->
-      (M (H := H') (core.option.Option u32));
-    get_contract_storage
-      `{H' : State.Trait}
-      {K R: Set}
-      `{parity_scale_codec.codec.Encode.Trait K}
-      `{ink_storage_traits.storage.Storable.Trait R}
-      :
-      (mut_ref Self) ->
-      (ref K) ->
-      (M (H := H') (ink_env.error.Result (core.option.Option R)));
-    take_contract_storage
-      `{H' : State.Trait}
-      {K R: Set}
-      `{parity_scale_codec.codec.Encode.Trait K}
-      `{ink_storage_traits.storage.Storable.Trait R}
-      :
-      (mut_ref Self) ->
-      (ref K) ->
-      (M (H := H') (ink_env.error.Result (core.option.Option R)));
-    contains_contract_storage
-      `{H' : State.Trait}
-      {K: Set}
-      `{parity_scale_codec.codec.Encode.Trait K}
-      :
-      (mut_ref Self) -> (ref K) -> (M (H := H') (core.option.Option u32));
-    clear_contract_storage
-      `{H' : State.Trait}
-      {K: Set}
-      `{parity_scale_codec.codec.Encode.Trait K}
-      :
-      (mut_ref Self) -> (ref K) -> (M (H := H') (core.option.Option u32));
-    decode_input
-      `{H' : State.Trait}
-      {T: Set}
-      `{parity_scale_codec.codec.Decode.Trait T}
-      :
-      (mut_ref Self) -> (M (H := H') (ink_env.error.Result T));
-    return_value
-      `{H' : State.Trait}
-      {R: Set}
-      `{parity_scale_codec.codec.Encode.Trait R}
-      :
-      (mut_ref Self) ->
-      ink_env.backend.ReturnFlags ->
-      (ref R) ->
-      (M (H := H') Empty_set);
-    debug_message
-      `{H' : State.Trait}
-      :
-      (mut_ref Self) -> (ref str) -> (M (H := H') unit);
-    hash_bytes
-      `{H' : State.Trait}
-      {H: Set}
-      `{ink_env.hash.CryptoHash.Trait H}
-      :
-      (mut_ref Self) ->
-      (ref (Slice u8)) ->
-      (mut_ref ink_env.hash.HashOutput.Type_) ->
-      (M (H := H') unit);
-    hash_encoded
-      `{H' : State.Trait}
-      {H T: Set}
-      `{ink_env.hash.CryptoHash.Trait H}
-      `{parity_scale_codec.codec.Encode.Trait T}
-      :
-      (mut_ref Self) ->
-      (ref T) ->
-      (mut_ref ink_env.hash.HashOutput.Type_) ->
-      (M (H := H') unit);
-    ecdsa_recover
-      `{H' : State.Trait}
-      :
-      (mut_ref Self) ->
-      (ref (list u8)) ->
-      (ref (list u8)) ->
-      (mut_ref (list u8)) ->
-      (M (H := H') (ink_env.error.Result unit));
-    ecdsa_to_eth_address
-      `{H' : State.Trait}
-      :
-      (mut_ref Self) ->
-      (ref (list u8)) ->
-      (mut_ref (list u8)) ->
-      (M (H := H') (ink_env.error.Result unit));
-    call_chain_extension
-      `{H' : State.Trait}
-      {I T E ErrorCode F D: Set}
-      `{parity_scale_codec.codec.Encode.Trait I}
-      `{parity_scale_codec.codec.Decode.Trait T}
-      `{core.convert.From.Trait E (T := ErrorCode)}
-      `{core.ops.function.FnOnce.Trait F (Args := u32)}
-      `{core.ops.function.FnOnce.Trait D (Args := ref (Slice u8))}
-      :
-      (mut_ref Self) ->
-      u32 ->
-      (ref I) ->
-      F ->
-      D ->
-      (M (H := H') (core.result.Result T E));
-    set_code_hash
-      `{H' : State.Trait}
-      :
-      (mut_ref Self) ->
-      (ref (Slice u8)) ->
-      (M (H := H') (ink_env.error.Result unit));
-  }.
-  
-  Global Instance Method_set_contract_storage `{H' : State.Trait} `(Trait)
-    : Notation.Dot "set_contract_storage" := {
-    Notation.dot
-      {K V : Set}
-      `{parity_scale_codec.codec.Encode.Trait K}
-      `{ink_storage_traits.storage.Storable.Trait V}
-      :=
-      set_contract_storage;
-  }.
-  Global Instance Method_get_contract_storage `{H' : State.Trait} `(Trait)
-    : Notation.Dot "get_contract_storage" := {
-    Notation.dot
-      {K R : Set}
-      `{parity_scale_codec.codec.Encode.Trait K}
-      `{ink_storage_traits.storage.Storable.Trait R}
-      :=
-      get_contract_storage;
-  }.
-  Global Instance Method_take_contract_storage `{H' : State.Trait} `(Trait)
-    : Notation.Dot "take_contract_storage" := {
-    Notation.dot
-      {K R : Set}
-      `{parity_scale_codec.codec.Encode.Trait K}
-      `{ink_storage_traits.storage.Storable.Trait R}
-      :=
-      take_contract_storage;
-  }.
-  Global Instance Method_contains_contract_storage `{H' : State.Trait} `(Trait)
-    : Notation.Dot "contains_contract_storage" := {
-    Notation.dot {K : Set} `{parity_scale_codec.codec.Encode.Trait K}
-      :=
-      contains_contract_storage;
-  }.
-  Global Instance Method_clear_contract_storage `{H' : State.Trait} `(Trait)
-    : Notation.Dot "clear_contract_storage" := {
-    Notation.dot {K : Set} `{parity_scale_codec.codec.Encode.Trait K}
-      :=
-      clear_contract_storage;
-  }.
-  Global Instance Method_decode_input `{H' : State.Trait} `(Trait)
-    : Notation.Dot "decode_input" := {
-    Notation.dot {T : Set} `{parity_scale_codec.codec.Decode.Trait T}
-      :=
-      decode_input;
-  }.
-  Global Instance Method_return_value `{H' : State.Trait} `(Trait)
-    : Notation.Dot "return_value" := {
-    Notation.dot {R : Set} `{parity_scale_codec.codec.Encode.Trait R}
-      :=
-      return_value;
-  }.
-  Global Instance Method_debug_message `{H' : State.Trait} `(Trait)
-    : Notation.Dot "debug_message" := {
-    Notation.dot := debug_message;
-  }.
-  Global Instance Method_hash_bytes `{H' : State.Trait} `(Trait)
-    : Notation.Dot "hash_bytes" := {
-    Notation.dot {H : Set} `{ink_env.hash.CryptoHash.Trait H} := hash_bytes;
-  }.
-  Global Instance Method_hash_encoded `{H' : State.Trait} `(Trait)
-    : Notation.Dot "hash_encoded" := {
-    Notation.dot
-      {H T : Set}
-      `{ink_env.hash.CryptoHash.Trait H}
-      `{parity_scale_codec.codec.Encode.Trait T}
-      :=
-      hash_encoded;
-  }.
-  Global Instance Method_ecdsa_recover `{H' : State.Trait} `(Trait)
-    : Notation.Dot "ecdsa_recover" := {
-    Notation.dot := ecdsa_recover;
-  }.
-  Global Instance Method_ecdsa_to_eth_address `{H' : State.Trait} `(Trait)
-    : Notation.Dot "ecdsa_to_eth_address" := {
-    Notation.dot := ecdsa_to_eth_address;
-  }.
-  Global Instance Method_call_chain_extension `{H' : State.Trait} `(Trait)
-    : Notation.Dot "call_chain_extension" := {
-    Notation.dot
-      {I T E ErrorCode F D : Set}
-      `{parity_scale_codec.codec.Encode.Trait I}
-      `{parity_scale_codec.codec.Decode.Trait T}
-      `{core.convert.From.Trait E (T := ErrorCode)}
-      `{core.ops.function.FnOnce.Trait F (Args := u32)}
-      `{core.ops.function.FnOnce.Trait D (Args := ref (Slice u8))}
-      :=
-      call_chain_extension;
-  }.
-  Global Instance Method_set_code_hash `{H' : State.Trait} `(Trait)
-    : Notation.Dot "set_code_hash" := {
-    Notation.dot := set_code_hash;
-  }.
-End EnvBackend.
-
-
-
-Module call_builder.
-  Module CallParams.
-    Section CallParams.
-      Context {E CallType Args R : Set}.
-      Context `{ink_env.types.Environment.Trait E}.
-      Unset Primitive Projections.
-      Record t : Set := {
-        call_type : CallType;
-        call_flags : ink_env.backend.CallFlags;
-        _return_type : ink_env.call.common.ReturnType R;
-        exec_input : ink_env.call.execution_input.ExecutionInput Args;
-        _phantom : core.marker.PhantomData (E);
-      }.
-      Global Set Primitive Projections.
-      
-      Global Instance Get_call_type : Notation.Dot "call_type" := {
-        Notation.dot '(Build_t x0 _ _ _ _) := x0;
-      }.
-      Global Instance Get_call_flags : Notation.Dot "call_flags" := {
-        Notation.dot '(Build_t _ x1 _ _ _) := x1;
-      }.
-      Global Instance Get__return_type : Notation.Dot "_return_type" := {
-        Notation.dot '(Build_t _ _ x2 _ _) := x2;
-      }.
-      Global Instance Get_exec_input : Notation.Dot "exec_input" := {
-        Notation.dot '(Build_t _ _ _ x3 _) := x3;
-      }.
-      Global Instance Get__phantom : Notation.Dot "_phantom" := {
-        Notation.dot '(Build_t _ _ _ _ x4) := x4;
-      }.
-    End CallParams.
-  End CallParams.
-  Definition CallParams
-      (E CallType Args R : Set)
-      `{ink_env.types.Environment.Trait E}
-      : Set :=
-    CallParams.t (E := E) (CallType := CallType) (Args := Args) (R := R).
-  
-  Module Call.
-    Section Call.
-      Context {E : Set}.
-      Context `{ink_env.types.Environment.Trait E}.
-      Unset Primitive Projections.
-      Record t : Set := {
-        callee : E::type["AccountId"];
-        gas_limit : ink_env.types.Gas;
-        transferred_value : E::type["Balance"];
-      }.
-      Global Set Primitive Projections.
-      
-      Global Instance Get_callee : Notation.Dot "callee" := {
-        Notation.dot '(Build_t x0 _ _) := x0;
-      }.
-      Global Instance Get_gas_limit : Notation.Dot "gas_limit" := {
-        Notation.dot '(Build_t _ x1 _) := x1;
-      }.
-      Global Instance Get_transferred_value
-        : Notation.Dot "transferred_value" := {
-        Notation.dot '(Build_t _ _ x2) := x2;
-      }.
-    End Call.
-  End Call.
-  Definition Call (E : Set) `{ink_env.types.Environment.Trait E} : Set :=
-    Call.t (E := E).
-  
-  Module CallBuilder.
-    Section CallBuilder.
-      Context {E CallType Args RetType : Set}.
-      Context `{ink_env.types.Environment.Trait E}.
-      Unset Primitive Projections.
-      Record t : Set := {
-        call_type : CallType;
-        call_flags : ink_env.backend.CallFlags;
-        exec_input : Args;
-        return_type : RetType;
-        _phantom : core.marker.PhantomData (E);
-      }.
-      Global Set Primitive Projections.
-      
-      Global Instance Get_call_type : Notation.Dot "call_type" := {
-        Notation.dot '(Build_t x0 _ _ _ _) := x0;
-      }.
-      Global Instance Get_call_flags : Notation.Dot "call_flags" := {
-        Notation.dot '(Build_t _ x1 _ _ _) := x1;
-      }.
-      Global Instance Get_exec_input : Notation.Dot "exec_input" := {
-        Notation.dot '(Build_t _ _ x2 _ _) := x2;
-      }.
-      Global Instance Get_return_type : Notation.Dot "return_type" := {
-        Notation.dot '(Build_t _ _ _ x3 _) := x3;
-      }.
-      Global Instance Get__phantom : Notation.Dot "_phantom" := {
-        Notation.dot '(Build_t _ _ _ _ x4) := x4;
-      }.
-    End CallBuilder.
-  End CallBuilder.
-  Definition CallBuilder
-      (E CallType Args RetType : Set)
-      `{ink_env.types.Environment.Trait E}
-      : Set :=
-    CallBuilder.t
-      (E := E)
-      (CallType := CallType)
-      (Args := Args)
-      (RetType := RetType).
-  
-  Parameter build_call :
-      forall `{H' : State.Trait} {E : Set} `{ink_env.types.Environment.Trait E},
-      M (H := H')
-          (ink_env.call.call_builder.CallBuilder
-            E
-            (ink_env.call.common.Unset_ (ink_env.call.call_builder.Call E))
-            (ink_env.call.common.Unset_
-              (ink_env.call.execution_input.ExecutionInput
-                ink_env.call.execution_input.EmptyArgumentList))
-            (ink_env.call.common.Unset_ (ink_env.call.common.ReturnType unit))).
-  
-  Module DelegateCall.
-    Section DelegateCall.
-      Context {E : Set}.
-      Context `{ink_env.types.Environment.Trait E}.
-      Unset Primitive Projections.
-      Record t : Set := {
-        code_hash : E::type["Hash"];
-      }.
-      Global Set Primitive Projections.
-      
-      Global Instance Get_code_hash : Notation.Dot "code_hash" := {
-        Notation.dot '(Build_t x0) := x0;
-      }.
-    End DelegateCall.
-  End DelegateCall.
-  Definition DelegateCall
-      (E : Set)
-      `{ink_env.types.Environment.Trait E}
-      : Set :=
-    DelegateCall.t (E := E).
-End call_builder.
+Definition Result (T : Set) : Set :=
+  core.result.Result T ink_env.backend_and_call_builder_and_error.Error.
 
 Module CallParams.
   Section CallParams.
@@ -2530,7 +2599,7 @@ Module CallParams.
     Unset Primitive Projections.
     Record t : Set := {
       call_type : CallType;
-      call_flags : ink_env.backend.CallFlags;
+      call_flags : ink_env.backend_and_call_builder_and_error.CallFlags;
       _return_type : ink_env.call.common.ReturnType R;
       exec_input : ink_env.call.execution_input.ExecutionInput Args;
       _phantom : core.marker.PhantomData (E);
@@ -2560,7 +2629,17 @@ Definition CallParams
     : Set :=
   CallParams.t (E := E) (CallType := CallType) (Args := Args) (R := R).
 
-
+Parameter build_call :
+    forall `{H' : State.Trait} {E : Set} `{ink_env.types.Environment.Trait E},
+    M (H := H')
+        (ink_env.backend_and_call_builder_and_error.CallBuilder
+          E
+          (ink_env.call.common.Unset_
+            (ink_env.backend_and_call_builder_and_error.Call E))
+          (ink_env.call.common.Unset_
+            (ink_env.call.execution_input.ExecutionInput
+              ink_env.call.execution_input.EmptyArgumentList))
+          (ink_env.call.common.Unset_ (ink_env.call.common.ReturnType unit))).
 
 Module Call.
   Section Call.
@@ -2614,7 +2693,7 @@ Module CallBuilder.
     Unset Primitive Projections.
     Record t : Set := {
       call_type : CallType;
-      call_flags : ink_env.backend.CallFlags;
+      call_flags : ink_env.backend_and_call_builder_and_error.CallFlags;
       exec_input : Args;
       return_type : RetType;
       _phantom : core.marker.PhantomData (E);
@@ -2647,6 +2726,618 @@ Definition CallBuilder
     (CallType := CallType)
     (Args := Args)
     (RetType := RetType).
+
+Module ReturnFlags.
+  Unset Primitive Projections.
+  Record t : Set := {
+    value : u32;
+  }.
+  Global Set Primitive Projections.
+  
+  Global Instance Get_value : Notation.Dot "value" := {
+    Notation.dot '(Build_t x0) := x0;
+  }.
+End ReturnFlags.
+Definition ReturnFlags : Set := ReturnFlags.t.
+
+Module CallFlags.
+  Unset Primitive Projections.
+  Record t : Set := {
+    forward_input : bool;
+    clone_input : bool;
+    tail_call : bool;
+    allow_reentry : bool;
+  }.
+  Global Set Primitive Projections.
+  
+  Global Instance Get_forward_input : Notation.Dot "forward_input" := {
+    Notation.dot '(Build_t x0 _ _ _) := x0;
+  }.
+  Global Instance Get_clone_input : Notation.Dot "clone_input" := {
+    Notation.dot '(Build_t _ x1 _ _) := x1;
+  }.
+  Global Instance Get_tail_call : Notation.Dot "tail_call" := {
+    Notation.dot '(Build_t _ _ x2 _) := x2;
+  }.
+  Global Instance Get_allow_reentry : Notation.Dot "allow_reentry" := {
+    Notation.dot '(Build_t _ _ _ x3) := x3;
+  }.
+End CallFlags.
+Definition CallFlags : Set := CallFlags.t.
+
+Module EnvBackend.
+  Class Trait (Self : Set) : Type := {
+    set_contract_storage
+      `{H' : State.Trait}
+      {K V: Set}
+      `{H'0 : parity_scale_codec.codec.Encode.Trait K}
+      `{H'1 : ink_storage_traits.storage.Storable.Trait V}
+      :
+      (mut_ref Self) ->
+      (ref K) ->
+      (ref V) ->
+      (M (H := H') (core.option.Option u32));
+    get_contract_storage
+      `{H' : State.Trait}
+      {K R: Set}
+      `{H'0 : parity_scale_codec.codec.Encode.Trait K}
+      `{H'1 : ink_storage_traits.storage.Storable.Trait R}
+      :
+      (mut_ref Self) ->
+      (ref K) ->
+      (M (H := H')
+        (ink_env.backend_and_call_builder_and_error.Result
+          (core.option.Option R)));
+    take_contract_storage
+      `{H' : State.Trait}
+      {K R: Set}
+      `{H'0 : parity_scale_codec.codec.Encode.Trait K}
+      `{H'1 : ink_storage_traits.storage.Storable.Trait R}
+      :
+      (mut_ref Self) ->
+      (ref K) ->
+      (M (H := H')
+        (ink_env.backend_and_call_builder_and_error.Result
+          (core.option.Option R)));
+    contains_contract_storage
+      `{H' : State.Trait}
+      {K: Set}
+      `{H'0 : parity_scale_codec.codec.Encode.Trait K}
+      :
+      (mut_ref Self) -> (ref K) -> (M (H := H') (core.option.Option u32));
+    clear_contract_storage
+      `{H' : State.Trait}
+      {K: Set}
+      `{H'0 : parity_scale_codec.codec.Encode.Trait K}
+      :
+      (mut_ref Self) -> (ref K) -> (M (H := H') (core.option.Option u32));
+    decode_input
+      `{H' : State.Trait}
+      {T: Set}
+      `{H'0 : parity_scale_codec.codec.Decode.Trait T}
+      :
+      (mut_ref Self) ->
+      (M (H := H') (ink_env.backend_and_call_builder_and_error.Result T));
+    return_value
+      `{H' : State.Trait}
+      {R: Set}
+      `{H'0 : parity_scale_codec.codec.Encode.Trait R}
+      :
+      (mut_ref Self) ->
+      ink_env.backend_and_call_builder_and_error.ReturnFlags ->
+      (ref R) ->
+      (M (H := H') Empty_set);
+    debug_message
+      `{H' : State.Trait}
+      :
+      (mut_ref Self) -> (ref str) -> (M (H := H') unit);
+    hash_bytes
+      `{H' : State.Trait}
+      {H: Set}
+      `{H'0 : ink_env.hash.CryptoHash.Trait H}
+      :
+      (mut_ref Self) ->
+      (ref (Slice u8)) ->
+      (mut_ref ink_env.hash.HashOutput.Type_) ->
+      (M (H := H') unit);
+    hash_encoded
+      `{H' : State.Trait}
+      {H T: Set}
+      `{H'0 : ink_env.hash.CryptoHash.Trait H}
+      `{H'1 : parity_scale_codec.codec.Encode.Trait T}
+      :
+      (mut_ref Self) ->
+      (ref T) ->
+      (mut_ref ink_env.hash.HashOutput.Type_) ->
+      (M (H := H') unit);
+    ecdsa_recover
+      `{H' : State.Trait}
+      :
+      (mut_ref Self) ->
+      (ref (list u8)) ->
+      (ref (list u8)) ->
+      (mut_ref (list u8)) ->
+      (M (H := H') (ink_env.backend_and_call_builder_and_error.Result unit));
+    ecdsa_to_eth_address
+      `{H' : State.Trait}
+      :
+      (mut_ref Self) ->
+      (ref (list u8)) ->
+      (mut_ref (list u8)) ->
+      (M (H := H') (ink_env.backend_and_call_builder_and_error.Result unit));
+    call_chain_extension
+      `{H' : State.Trait}
+      {I T E ErrorCode F D: Set}
+      `{H'0 : parity_scale_codec.codec.Encode.Trait I}
+      `{H'1 : parity_scale_codec.codec.Decode.Trait T}
+      `{H'2 : core.convert.From.Trait E (T := ErrorCode)}
+      `{H'3 : core.ops.function.FnOnce.Trait F (Args := u32)}
+      `{H'4 : core.ops.function.FnOnce.Trait D (Args := ref (Slice u8))}
+      :
+      (mut_ref Self) ->
+      u32 ->
+      (ref I) ->
+      F ->
+      D ->
+      (M (H := H') (core.result.Result T E));
+    set_code_hash
+      `{H' : State.Trait}
+      :
+      (mut_ref Self) ->
+      (ref (Slice u8)) ->
+      (M (H := H') (ink_env.backend_and_call_builder_and_error.Result unit));
+  }.
+  
+  Global Instance Method_set_contract_storage `{H' : State.Trait} `(Trait)
+    : Notation.Dot "set_contract_storage" := {
+    Notation.dot
+      {K V : Set}
+      `{H'0 : parity_scale_codec.codec.Encode.Trait K}
+      `{H'1 : ink_storage_traits.storage.Storable.Trait V}
+      :=
+      set_contract_storage (K := K) (V := V) (H'0 := H'0) (H'1 := H'1);
+  }.
+  Global Instance Method_get_contract_storage `{H' : State.Trait} `(Trait)
+    : Notation.Dot "get_contract_storage" := {
+    Notation.dot
+      {K R : Set}
+      `{H'0 : parity_scale_codec.codec.Encode.Trait K}
+      `{H'1 : ink_storage_traits.storage.Storable.Trait R}
+      :=
+      get_contract_storage (K := K) (R := R) (H'0 := H'0) (H'1 := H'1);
+  }.
+  Global Instance Method_take_contract_storage `{H' : State.Trait} `(Trait)
+    : Notation.Dot "take_contract_storage" := {
+    Notation.dot
+      {K R : Set}
+      `{H'0 : parity_scale_codec.codec.Encode.Trait K}
+      `{H'1 : ink_storage_traits.storage.Storable.Trait R}
+      :=
+      take_contract_storage (K := K) (R := R) (H'0 := H'0) (H'1 := H'1);
+  }.
+  Global Instance Method_contains_contract_storage `{H' : State.Trait} `(Trait)
+    : Notation.Dot "contains_contract_storage" := {
+    Notation.dot {K : Set} `{H'0 : parity_scale_codec.codec.Encode.Trait K}
+      :=
+      contains_contract_storage (K := K) (H'0 := H'0);
+  }.
+  Global Instance Method_clear_contract_storage `{H' : State.Trait} `(Trait)
+    : Notation.Dot "clear_contract_storage" := {
+    Notation.dot {K : Set} `{H'0 : parity_scale_codec.codec.Encode.Trait K}
+      :=
+      clear_contract_storage (K := K) (H'0 := H'0);
+  }.
+  Global Instance Method_decode_input `{H' : State.Trait} `(Trait)
+    : Notation.Dot "decode_input" := {
+    Notation.dot {T : Set} `{H'0 : parity_scale_codec.codec.Decode.Trait T}
+      :=
+      decode_input (T := T) (H'0 := H'0);
+  }.
+  Global Instance Method_return_value `{H' : State.Trait} `(Trait)
+    : Notation.Dot "return_value" := {
+    Notation.dot {R : Set} `{H'0 : parity_scale_codec.codec.Encode.Trait R}
+      :=
+      return_value (R := R) (H'0 := H'0);
+  }.
+  Global Instance Method_debug_message `{H' : State.Trait} `(Trait)
+    : Notation.Dot "debug_message" := {
+    Notation.dot := debug_message;
+  }.
+  Global Instance Method_hash_bytes `{H' : State.Trait} `(Trait)
+    : Notation.Dot "hash_bytes" := {
+    Notation.dot {H : Set} `{H'0 : ink_env.hash.CryptoHash.Trait H}
+      :=
+      hash_bytes (H := H) (H'0 := H'0);
+  }.
+  Global Instance Method_hash_encoded `{H' : State.Trait} `(Trait)
+    : Notation.Dot "hash_encoded" := {
+    Notation.dot
+      {H T : Set}
+      `{H'0 : ink_env.hash.CryptoHash.Trait H}
+      `{H'1 : parity_scale_codec.codec.Encode.Trait T}
+      :=
+      hash_encoded (H := H) (T := T) (H'0 := H'0) (H'1 := H'1);
+  }.
+  Global Instance Method_ecdsa_recover `{H' : State.Trait} `(Trait)
+    : Notation.Dot "ecdsa_recover" := {
+    Notation.dot := ecdsa_recover;
+  }.
+  Global Instance Method_ecdsa_to_eth_address `{H' : State.Trait} `(Trait)
+    : Notation.Dot "ecdsa_to_eth_address" := {
+    Notation.dot := ecdsa_to_eth_address;
+  }.
+  Global Instance Method_call_chain_extension `{H' : State.Trait} `(Trait)
+    : Notation.Dot "call_chain_extension" := {
+    Notation.dot
+      {I T E ErrorCode F D : Set}
+      `{H'0 : parity_scale_codec.codec.Encode.Trait I}
+      `{H'1 : parity_scale_codec.codec.Decode.Trait T}
+      `{H'2 : core.convert.From.Trait E (T := ErrorCode)}
+      `{H'3 : core.ops.function.FnOnce.Trait F (Args := u32)}
+      `{H'4 : core.ops.function.FnOnce.Trait D (Args := ref (Slice u8))}
+      :=
+      call_chain_extension
+          (I := I)
+          (T := T)
+          (E := E)
+          (ErrorCode := ErrorCode)
+          (F := F)
+          (D := D)
+        (H'0 := H'0)
+        (H'1 := H'1)
+        (H'2 := H'2)
+        (H'3 := H'3)
+        (H'4 := H'4);
+  }.
+  Global Instance Method_set_code_hash `{H' : State.Trait} `(Trait)
+    : Notation.Dot "set_code_hash" := {
+    Notation.dot := set_code_hash;
+  }.
+End EnvBackend.
+
+Module TypedEnvBackend.
+  Class Trait
+      (Self : Set)
+        `{ink_env.backend_and_call_builder_and_error.EnvBackend.Trait Self} :
+      Type := {
+    caller
+      `{H' : State.Trait}
+      {E: Set}
+      `{H'0 : ink_env.types.Environment.Trait E}
+      :
+      (mut_ref Self) -> (M (H := H') E::type["AccountId"]);
+    transferred_value
+      `{H' : State.Trait}
+      {E: Set}
+      `{H'0 : ink_env.types.Environment.Trait E}
+      :
+      (mut_ref Self) -> (M (H := H') E::type["Balance"]);
+    weight_to_fee
+      `{H' : State.Trait}
+      {E: Set}
+      `{H'0 : ink_env.types.Environment.Trait E}
+      :
+      (mut_ref Self) -> u64 -> (M (H := H') E::type["Balance"]);
+    gas_left
+      `{H' : State.Trait}
+      {E: Set}
+      `{H'0 : ink_env.types.Environment.Trait E}
+      :
+      (mut_ref Self) -> (M (H := H') u64);
+    block_timestamp
+      `{H' : State.Trait}
+      {E: Set}
+      `{H'0 : ink_env.types.Environment.Trait E}
+      :
+      (mut_ref Self) -> (M (H := H') E::type["Timestamp"]);
+    account_id
+      `{H' : State.Trait}
+      {E: Set}
+      `{H'0 : ink_env.types.Environment.Trait E}
+      :
+      (mut_ref Self) -> (M (H := H') E::type["AccountId"]);
+    balance
+      `{H' : State.Trait}
+      {E: Set}
+      `{H'0 : ink_env.types.Environment.Trait E}
+      :
+      (mut_ref Self) -> (M (H := H') E::type["Balance"]);
+    block_number
+      `{H' : State.Trait}
+      {E: Set}
+      `{H'0 : ink_env.types.Environment.Trait E}
+      :
+      (mut_ref Self) -> (M (H := H') E::type["BlockNumber"]);
+    minimum_balance
+      `{H' : State.Trait}
+      {E: Set}
+      `{H'0 : ink_env.types.Environment.Trait E}
+      :
+      (mut_ref Self) -> (M (H := H') E::type["Balance"]);
+    emit_event
+      `{H' : State.Trait}
+      {E Event: Set}
+      `{H'0 : ink_env.types.Environment.Trait E}
+      `{H'1 : ink_env.topics.Topics.Trait Event}
+      `{H'2 : parity_scale_codec.codec.Encode.Trait Event}
+      :
+      (mut_ref Self) -> Event -> (M (H := H') unit);
+    invoke_contract
+      `{H' : State.Trait}
+      {E Args R: Set}
+      `{H'0 : ink_env.types.Environment.Trait E}
+      `{H'1 : parity_scale_codec.codec.Encode.Trait Args}
+      `{H'2 : parity_scale_codec.codec.Decode.Trait R}
+      :
+      (mut_ref Self) ->
+      (ref
+        (ink_env.backend_and_call_builder_and_error.CallParams
+          E
+          (ink_env.backend_and_call_builder_and_error.Call E)
+          Args
+          R)) ->
+      (M (H := H')
+        (ink_env.backend_and_call_builder_and_error.Result
+          (ink_primitives.MessageResult R)));
+    invoke_contract_delegate
+      `{H' : State.Trait}
+      {E Args R: Set}
+      `{H'0 : ink_env.types.Environment.Trait E}
+      `{H'1 : parity_scale_codec.codec.Encode.Trait Args}
+      `{H'2 : parity_scale_codec.codec.Decode.Trait R}
+      :
+      (mut_ref Self) ->
+      (ref
+        (ink_env.backend_and_call_builder_and_error.CallParams
+          E
+          (ink_env.backend_and_call_builder_and_error.DelegateCall E)
+          Args
+          R)) ->
+      (M (H := H')
+        (ink_env.backend_and_call_builder_and_error.Result
+          (ink_primitives.MessageResult R)));
+    instantiate_contract
+      `{H' : State.Trait}
+      {E ContractRef Args Salt R: Set}
+      `{H'0 : ink_env.types.Environment.Trait E}
+      `{H'1
+        :
+        ink_env.call.create_builder.FromAccountId.Trait ContractRef (T := E)}
+      `{H'2 : parity_scale_codec.codec.Encode.Trait Args}
+      `{H'3 : core.convert.AsRef.Trait Salt (T := Slice u8)}
+      `{H'4
+        :
+        ink_env.call.create_builder.ConstructorReturnType.Trait R
+          (C := ContractRef)}
+      :
+      (mut_ref Self) ->
+      (ref
+        (ink_env.call.create_builder.CreateParams E ContractRef Args Salt R)) ->
+      (M (H := H')
+        (ink_env.backend_and_call_builder_and_error.Result
+          (ink_primitives.ConstructorResult
+            ink_env.call.create_builder.ConstructorReturnType.Output)));
+    terminate_contract
+      `{H' : State.Trait}
+      {E: Set}
+      `{H'0 : ink_env.types.Environment.Trait E}
+      :
+      (mut_ref Self) -> E::type["AccountId"] -> (M (H := H') Empty_set);
+    transfer
+      `{H' : State.Trait}
+      {E: Set}
+      `{H'0 : ink_env.types.Environment.Trait E}
+      :
+      (mut_ref Self) ->
+      E::type["AccountId"] ->
+      E::type["Balance"] ->
+      (M (H := H') (ink_env.backend_and_call_builder_and_error.Result unit));
+    is_contract
+      `{H' : State.Trait}
+      {E: Set}
+      `{H'0 : ink_env.types.Environment.Trait E}
+      :
+      (mut_ref Self) -> (ref E::type["AccountId"]) -> (M (H := H') bool);
+    caller_is_origin
+      `{H' : State.Trait}
+      {E: Set}
+      `{H'0 : ink_env.types.Environment.Trait E}
+      :
+      (mut_ref Self) -> (M (H := H') bool);
+    code_hash
+      `{H' : State.Trait}
+      {E: Set}
+      `{H'0 : ink_env.types.Environment.Trait E}
+      :
+      (mut_ref Self) ->
+      (ref E::type["AccountId"]) ->
+      (M (H := H')
+        (ink_env.backend_and_call_builder_and_error.Result E::type["Hash"]));
+    own_code_hash
+      `{H' : State.Trait}
+      {E: Set}
+      `{H'0 : ink_env.types.Environment.Trait E}
+      :
+      (mut_ref Self) ->
+      (M (H := H')
+        (ink_env.backend_and_call_builder_and_error.Result E::type["Hash"]));
+    call_runtime
+      `{H' : State.Trait}
+      {E Call: Set}
+      `{H'0 : ink_env.types.Environment.Trait E}
+      `{H'1 : parity_scale_codec.codec.Encode.Trait Call}
+      :
+      (mut_ref Self) ->
+      (ref Call) ->
+      (M (H := H') (ink_env.backend_and_call_builder_and_error.Result unit));
+  }.
+  
+  Global Instance Method_caller `{H' : State.Trait} `(Trait)
+    : Notation.Dot "caller" := {
+    Notation.dot {E : Set} `{H'0 : ink_env.types.Environment.Trait E}
+      :=
+      caller (E := E) (H'0 := H'0);
+  }.
+  Global Instance Method_transferred_value `{H' : State.Trait} `(Trait)
+    : Notation.Dot "transferred_value" := {
+    Notation.dot {E : Set} `{H'0 : ink_env.types.Environment.Trait E}
+      :=
+      transferred_value (E := E) (H'0 := H'0);
+  }.
+  Global Instance Method_weight_to_fee `{H' : State.Trait} `(Trait)
+    : Notation.Dot "weight_to_fee" := {
+    Notation.dot {E : Set} `{H'0 : ink_env.types.Environment.Trait E}
+      :=
+      weight_to_fee (E := E) (H'0 := H'0);
+  }.
+  Global Instance Method_gas_left `{H' : State.Trait} `(Trait)
+    : Notation.Dot "gas_left" := {
+    Notation.dot {E : Set} `{H'0 : ink_env.types.Environment.Trait E}
+      :=
+      gas_left (E := E) (H'0 := H'0);
+  }.
+  Global Instance Method_block_timestamp `{H' : State.Trait} `(Trait)
+    : Notation.Dot "block_timestamp" := {
+    Notation.dot {E : Set} `{H'0 : ink_env.types.Environment.Trait E}
+      :=
+      block_timestamp (E := E) (H'0 := H'0);
+  }.
+  Global Instance Method_account_id `{H' : State.Trait} `(Trait)
+    : Notation.Dot "account_id" := {
+    Notation.dot {E : Set} `{H'0 : ink_env.types.Environment.Trait E}
+      :=
+      account_id (E := E) (H'0 := H'0);
+  }.
+  Global Instance Method_balance `{H' : State.Trait} `(Trait)
+    : Notation.Dot "balance" := {
+    Notation.dot {E : Set} `{H'0 : ink_env.types.Environment.Trait E}
+      :=
+      balance (E := E) (H'0 := H'0);
+  }.
+  Global Instance Method_block_number `{H' : State.Trait} `(Trait)
+    : Notation.Dot "block_number" := {
+    Notation.dot {E : Set} `{H'0 : ink_env.types.Environment.Trait E}
+      :=
+      block_number (E := E) (H'0 := H'0);
+  }.
+  Global Instance Method_minimum_balance `{H' : State.Trait} `(Trait)
+    : Notation.Dot "minimum_balance" := {
+    Notation.dot {E : Set} `{H'0 : ink_env.types.Environment.Trait E}
+      :=
+      minimum_balance (E := E) (H'0 := H'0);
+  }.
+  Global Instance Method_emit_event `{H' : State.Trait} `(Trait)
+    : Notation.Dot "emit_event" := {
+    Notation.dot
+      {E Event : Set}
+      `{H'0 : ink_env.types.Environment.Trait E}
+      `{H'1 : ink_env.topics.Topics.Trait Event}
+      `{H'2 : parity_scale_codec.codec.Encode.Trait Event}
+      :=
+      emit_event (E := E) (Event := Event)
+        (H'0 := H'0)
+        (H'1 := H'1)
+        (H'2 := H'2);
+  }.
+  Global Instance Method_invoke_contract `{H' : State.Trait} `(Trait)
+    : Notation.Dot "invoke_contract" := {
+    Notation.dot
+      {E Args R : Set}
+      `{H'0 : ink_env.types.Environment.Trait E}
+      `{H'1 : parity_scale_codec.codec.Encode.Trait Args}
+      `{H'2 : parity_scale_codec.codec.Decode.Trait R}
+      :=
+      invoke_contract (E := E) (Args := Args) (R := R)
+        (H'0 := H'0)
+        (H'1 := H'1)
+        (H'2 := H'2);
+  }.
+  Global Instance Method_invoke_contract_delegate `{H' : State.Trait} `(Trait)
+    : Notation.Dot "invoke_contract_delegate" := {
+    Notation.dot
+      {E Args R : Set}
+      `{H'0 : ink_env.types.Environment.Trait E}
+      `{H'1 : parity_scale_codec.codec.Encode.Trait Args}
+      `{H'2 : parity_scale_codec.codec.Decode.Trait R}
+      :=
+      invoke_contract_delegate (E := E) (Args := Args) (R := R)
+        (H'0 := H'0)
+        (H'1 := H'1)
+        (H'2 := H'2);
+  }.
+  Global Instance Method_instantiate_contract `{H' : State.Trait} `(Trait)
+    : Notation.Dot "instantiate_contract" := {
+    Notation.dot
+      {E ContractRef Args Salt R : Set}
+      `{H'0 : ink_env.types.Environment.Trait E}
+      `{H'1
+        :
+        ink_env.call.create_builder.FromAccountId.Trait ContractRef (T := E)}
+      `{H'2 : parity_scale_codec.codec.Encode.Trait Args}
+      `{H'3 : core.convert.AsRef.Trait Salt (T := Slice u8)}
+      `{H'4
+        :
+        ink_env.call.create_builder.ConstructorReturnType.Trait R
+          (C := ContractRef)}
+      :=
+      instantiate_contract
+          (E := E)
+          (ContractRef := ContractRef)
+          (Args := Args)
+          (Salt := Salt)
+          (R := R)
+        (H'0 := H'0)
+        (H'1 := H'1)
+        (H'2 := H'2)
+        (H'3 := H'3)
+        (H'4 := H'4);
+  }.
+  Global Instance Method_terminate_contract `{H' : State.Trait} `(Trait)
+    : Notation.Dot "terminate_contract" := {
+    Notation.dot {E : Set} `{H'0 : ink_env.types.Environment.Trait E}
+      :=
+      terminate_contract (E := E) (H'0 := H'0);
+  }.
+  Global Instance Method_transfer `{H' : State.Trait} `(Trait)
+    : Notation.Dot "transfer" := {
+    Notation.dot {E : Set} `{H'0 : ink_env.types.Environment.Trait E}
+      :=
+      transfer (E := E) (H'0 := H'0);
+  }.
+  Global Instance Method_is_contract `{H' : State.Trait} `(Trait)
+    : Notation.Dot "is_contract" := {
+    Notation.dot {E : Set} `{H'0 : ink_env.types.Environment.Trait E}
+      :=
+      is_contract (E := E) (H'0 := H'0);
+  }.
+  Global Instance Method_caller_is_origin `{H' : State.Trait} `(Trait)
+    : Notation.Dot "caller_is_origin" := {
+    Notation.dot {E : Set} `{H'0 : ink_env.types.Environment.Trait E}
+      :=
+      caller_is_origin (E := E) (H'0 := H'0);
+  }.
+  Global Instance Method_code_hash `{H' : State.Trait} `(Trait)
+    : Notation.Dot "code_hash" := {
+    Notation.dot {E : Set} `{H'0 : ink_env.types.Environment.Trait E}
+      :=
+      code_hash (E := E) (H'0 := H'0);
+  }.
+  Global Instance Method_own_code_hash `{H' : State.Trait} `(Trait)
+    : Notation.Dot "own_code_hash" := {
+    Notation.dot {E : Set} `{H'0 : ink_env.types.Environment.Trait E}
+      :=
+      own_code_hash (E := E) (H'0 := H'0);
+  }.
+  Global Instance Method_call_runtime `{H' : State.Trait} `(Trait)
+    : Notation.Dot "call_runtime" := {
+    Notation.dot
+      {E Call : Set}
+      `{H'0 : ink_env.types.Environment.Trait E}
+      `{H'1 : parity_scale_codec.codec.Encode.Trait Call}
+      :=
+      call_runtime (E := E) (Call := Call) (H'0 := H'0) (H'1 := H'1);
+  }.
+End TypedEnvBackend.
 
 Module common.
   Module ReturnType.
@@ -2703,7 +3394,7 @@ Module common.
       unwrap_or_else
         `{H' : State.Trait}
         {F: Set}
-        `{core.ops.function.FnOnce.Trait F (Args := unit)}
+        `{H'0 : core.ops.function.FnOnce.Trait F (Args := unit)}
         :
         Self -> F -> (M (H := H') Output);
     }.
@@ -2714,9 +3405,11 @@ Module common.
     }.
     Global Instance Method_unwrap_or_else `{H' : State.Trait} `(Trait)
       : Notation.Dot "unwrap_or_else" := {
-      Notation.dot {F : Set} `{core.ops.function.FnOnce.Trait F (Args := unit)}
+      Notation.dot
+        {F : Set}
+        `{H'0 : core.ops.function.FnOnce.Trait F (Args := unit)}
         :=
-        unwrap_or_else;
+        unwrap_or_else (F := F) (H'0 := H'0);
     }.
   End Unwrap.
 End common.
@@ -2775,7 +3468,7 @@ Module Unwrap.
     unwrap_or_else
       `{H' : State.Trait}
       {F: Set}
-      `{core.ops.function.FnOnce.Trait F (Args := unit)}
+      `{H'0 : core.ops.function.FnOnce.Trait F (Args := unit)}
       :
       Self -> F -> (M (H := H') Output);
   }.
@@ -2786,9 +3479,11 @@ Module Unwrap.
   }.
   Global Instance Method_unwrap_or_else `{H' : State.Trait} `(Trait)
     : Notation.Dot "unwrap_or_else" := {
-    Notation.dot {F : Set} `{core.ops.function.FnOnce.Trait F (Args := unit)}
+    Notation.dot
+      {F : Set}
+      `{H'0 : core.ops.function.FnOnce.Trait F (Args := unit)}
       :=
-      unwrap_or_else;
+      unwrap_or_else (F := F) (H'0 := H'0);
   }.
 End Unwrap.
 
@@ -3522,7 +4217,30 @@ Module ContractReference.
   }.
 End ContractReference.
 
-
+Module OnInstance.
+  Class Trait
+      (Self : Set)
+        `{ink_env.backend_and_call_builder_and_error.EnvBackend.Trait Self}
+        `{ink_env.backend_and_call_builder_and_error.TypedEnvBackend.Trait
+              Self} :
+      Type := {
+    on_instance
+      `{H' : State.Trait}
+      {F R: Set}
+      `{H'0 : core.ops.function.FnOnce.Trait F (Args := mut_ref Self)}
+      :
+      F -> (M (H := H') R);
+  }.
+  
+  Global Instance Method_on_instance `{H' : State.Trait} `(Trait)
+    : Notation.Dot "on_instance" := {
+    Notation.dot
+      {F R : Set}
+      `{H'0 : core.ops.function.FnOnce.Trait F (Args := mut_ref Self)}
+      :=
+      on_instance (F := F) (R := R) (H'0 := H'0);
+  }.
+End OnInstance.
 
 Module off_chain.
   Module call_data.
@@ -3963,7 +4681,8 @@ Parameter set_account_balance :
 Parameter get_account_balance :
     forall `{H' : State.Trait} {T : Set} `{ink_env.types.Environment.Trait T},
     T::type["AccountId"] ->
-      M (H := H') (ink_env.error.Result T::type["Balance"]).
+      M (H := H')
+        (ink_env.backend_and_call_builder_and_error.Result T::type["Balance"]).
 
 
 
@@ -4024,7 +4743,8 @@ Parameter transfer_in :
 
 Parameter count_used_storage_cells :
     forall `{H' : State.Trait} {T : Set} `{ink_env.types.Environment.Trait T},
-    (ref T::type["AccountId"]) -> M (H := H') (ink_env.error.Result usize).
+    (ref T::type["AccountId"]) ->
+      M (H := H') (ink_env.backend_and_call_builder_and_error.Result usize).
 
 Parameter set_block_timestamp :
     forall `{H' : State.Trait} {T : Set} `{ink_env.types.Environment.Trait T},
@@ -4034,7 +4754,16 @@ Parameter set_block_number :
     forall `{H' : State.Trait} {T : Set} `{ink_env.types.Environment.Trait T},
     T::type["BlockNumber"] -> M (H := H') unit.
 
-
+Parameter run_test :
+    forall
+      `{H' : State.Trait}
+      {T F : Set}
+      `{ink_env.types.Environment.Trait T}
+      `{core.ops.function.FnOnce.Trait F
+          (Args := ink_env.engine.off_chain.test_api.DefaultAccounts T)}
+      `{core.convert.From.Trait ink_env.types.Environment.AccountId
+          (T := list u8)},
+    F -> M (H := H') (ink_env.backend_and_call_builder_and_error.Result unit).
 
 
 
@@ -4117,27 +4846,6 @@ Module AccountError.
 End AccountError.
 Definition AccountError := AccountError.t.
 
-Module Error.
-  Inductive t : Set :=
-  | Decode (_ : parity_scale_codec.error.Error)
-  | OffChain (_ : ink_env.engine.off_chain.OffChainError)
-  | CalleeTrapped
-  | CalleeReverted
-  | KeyNotFound
-  | _BelowSubsistenceThreshold
-  | TransferFailed
-  | _EndowmentTooLow
-  | CodeNotFound
-  | NotCallable
-  | Unknown
-  | LoggingDisabled
-  | CallRuntimeFailed
-  | EcdsaRecoveryFailed.
-End Error.
-Definition Error := Error.t.
-
-Definition Result (T : Set) : Set := core.result.Result T ink_env.error.Error.
-
 Module HashOutput.
   Class Trait (Self : Set) `{ink_env.hash.private.Sealed.Trait Self} : Type := {
     Type_ : Set;
@@ -4212,7 +4920,7 @@ Module TopicsBuilderBackend.
     push_topic
       `{H' : State.Trait}
       {T: Set}
-      `{parity_scale_codec.codec.Encode.Trait T}
+      `{H'0 : parity_scale_codec.codec.Encode.Trait T}
       :
       (mut_ref Self) -> (ref T) -> (M (H := H') unit);
     output `{H' : State.Trait} : Self -> (M (H := H') Output);
@@ -4228,9 +4936,9 @@ Module TopicsBuilderBackend.
   }.
   Global Instance Method_push_topic `{H' : State.Trait} `(Trait)
     : Notation.Dot "push_topic" := {
-    Notation.dot {T : Set} `{parity_scale_codec.codec.Encode.Trait T}
+    Notation.dot {T : Set} `{H'0 : parity_scale_codec.codec.Encode.Trait T}
       :=
-      push_topic;
+      push_topic (T := T) (H'0 := H'0);
   }.
   Global Instance Method_output `{H' : State.Trait} `(Trait)
     : Notation.Dot "output" := {
@@ -4306,8 +5014,8 @@ Module Topics.
     topics
       `{H' : State.Trait}
       {E B: Set}
-      `{ink_env.types.Environment.Trait E}
-      `{ink_env.topics.TopicsBuilderBackend.Trait B (E := E)}
+      `{H'0 : ink_env.types.Environment.Trait E}
+      `{H'1 : ink_env.topics.TopicsBuilderBackend.Trait B (E := E)}
       :
       (ref Self) ->
       (ink_env.topics.TopicsBuilder ink_env.topics.state.Uninit E B) ->
@@ -4322,10 +5030,10 @@ Module Topics.
     : Notation.Dot "topics" := {
     Notation.dot
       {E B : Set}
-      `{ink_env.types.Environment.Trait E}
-      `{ink_env.topics.TopicsBuilderBackend.Trait B (E := E)}
+      `{H'0 : ink_env.types.Environment.Trait E}
+      `{H'1 : ink_env.topics.TopicsBuilderBackend.Trait B (E := E)}
       :=
-      topics;
+      topics (E := E) (B := B) (H'0 := H'0) (H'1 := H'1);
   }.
 End Topics.
 
