CoqOfRust/ink/erc20.v
@@ -3038,7 +3038,9 @@ Module
         end in
       let* _ :=
         let* α0 := output_result.["is_err"] in
-        let* α1 := ink_env.backend.ReturnFlags::["new_with_reverted"] α0 in
+        let* α1 :=
+          ink_env.backend_and_call_builder_and_error.ReturnFlags::["new_with_reverted"]
+            α0 in
         let* α2 := output_result.["map"] (fun _ => Pure tt) in
         let* α3 := ink_primitives.ConstructorResult::["Ok"] α2 in
         ink_env.api.return_value α1 (addr_of α3) in
@@ -3374,7 +3376,8 @@ Module
           else
             Pure tt in
         let* α0 :=
-          ink_env.backend.ReturnFlags::["new_with_reverted"] is_reverted in
+          ink_env.backend_and_call_builder_and_error.ReturnFlags::["new_with_reverted"]
+            is_reverted in
         let* α1 := ink_primitives.MessageResult::["Ok"] result in
         ink_env.api.return_value α0 (addr_of α1)
       | Message1.Build_t input =>
@@ -3440,7 +3443,8 @@ Module
           else
             Pure tt in
         let* α0 :=
-          ink_env.backend.ReturnFlags::["new_with_reverted"] is_reverted in
+          ink_env.backend_and_call_builder_and_error.ReturnFlags::["new_with_reverted"]
+            is_reverted in
         let* α1 := ink_primitives.MessageResult::["Ok"] result in
         ink_env.api.return_value α0 (addr_of α1)
       | Message2.Build_t input =>
@@ -3506,7 +3510,8 @@ Module
           else
             Pure tt in
         let* α0 :=
-          ink_env.backend.ReturnFlags::["new_with_reverted"] is_reverted in
+          ink_env.backend_and_call_builder_and_error.ReturnFlags::["new_with_reverted"]
+            is_reverted in
         let* α1 := ink_primitives.MessageResult::["Ok"] result in
         ink_env.api.return_value α0 (addr_of α1)
       | Message3.Build_t input =>
@@ -3572,7 +3577,8 @@ Module
           else
             Pure tt in
         let* α0 :=
-          ink_env.backend.ReturnFlags::["new_with_reverted"] is_reverted in
+          ink_env.backend_and_call_builder_and_error.ReturnFlags::["new_with_reverted"]
+            is_reverted in
         let* α1 := ink_primitives.MessageResult::["Ok"] result in
         ink_env.api.return_value α0 (addr_of α1)
       | Message4.Build_t input =>
@@ -3638,7 +3644,8 @@ Module
           else
             Pure tt in
         let* α0 :=
-          ink_env.backend.ReturnFlags::["new_with_reverted"] is_reverted in
+          ink_env.backend_and_call_builder_and_error.ReturnFlags::["new_with_reverted"]
+            is_reverted in
         let* α1 := ink_primitives.MessageResult::["Ok"] result in
         ink_env.api.return_value α0 (addr_of α1)
       | Message5.Build_t input =>
@@ -3704,7 +3711,8 @@ Module
           else
             Pure tt in
         let* α0 :=
-          ink_env.backend.ReturnFlags::["new_with_reverted"] is_reverted in
+          ink_env.backend_and_call_builder_and_error.ReturnFlags::["new_with_reverted"]
+            is_reverted in
         let* α1 := ink_primitives.MessageResult::["Ok"] result in
         ink_env.api.return_value α0 (addr_of α1)
       end in
@@ -4471,16 +4479,17 @@ Module Impl_erc20_erc20___CallBuilder_18.
       (self : ref Self)
       :
         M (H := H')
-          (ink_env.call.call_builder.CallBuilder
+          (ink_env.backend_and_call_builder_and_error.CallBuilder
             erc20.erc20.Environment
             (ink_env.call.common.Set_
-              (ink_env.call.call_builder.Call erc20.erc20.Environment))
+              (ink_env.backend_and_call_builder_and_error.Call
+                erc20.erc20.Environment))
             (ink_env.call.common.Set_
               (ink_env.call.execution_input.ExecutionInput
                 ink_env.call.execution_input.EmptyArgumentList))
             (ink_env.call.common.Set_
               (ink_env.call.common.ReturnType erc20.erc20.Balance))) :=
-    let* α0 := ink_env.call.call_builder.build_call in
+    let* α0 := ink_env.backend_and_call_builder_and_error.build_call in
     let* α1 := ink.contract_ref.ToAccountId.to_account_id self in
     let* α2 := α0.["call"] α1 in
     let* α3 := ink_env.call.selector.Selector::["new"] [ 219; 99; 117; 168 ] in
@@ -4499,10 +4508,11 @@ Module Impl_erc20_erc20___CallBuilder_18.
       (__ink_binding_0 : erc20.erc20.AccountId)
       :
         M (H := H')
-          (ink_env.call.call_builder.CallBuilder
+          (ink_env.backend_and_call_builder_and_error.CallBuilder
             erc20.erc20.Environment
             (ink_env.call.common.Set_
-              (ink_env.call.call_builder.Call erc20.erc20.Environment))
+              (ink_env.backend_and_call_builder_and_error.Call
+                erc20.erc20.Environment))
             (ink_env.call.common.Set_
               (ink_env.call.execution_input.ExecutionInput
                 (ink_env.call.execution_input.ArgumentList
@@ -4510,7 +4520,7 @@ Module Impl_erc20_erc20___CallBuilder_18.
                   ink_env.call.execution_input.EmptyArgumentList)))
             (ink_env.call.common.Set_
               (ink_env.call.common.ReturnType erc20.erc20.Balance))) :=
-    let* α0 := ink_env.call.call_builder.build_call in
+    let* α0 := ink_env.backend_and_call_builder_and_error.build_call in
     let* α1 := ink.contract_ref.ToAccountId.to_account_id self in
     let* α2 := α0.["call"] α1 in
     let* α3 := ink_env.call.selector.Selector::["new"] [ 15; 117; 90; 86 ] in
@@ -4531,10 +4541,11 @@ Module Impl_erc20_erc20___CallBuilder_18.
       (__ink_binding_1 : erc20.erc20.AccountId)
       :
         M (H := H')
-          (ink_env.call.call_builder.CallBuilder
+          (ink_env.backend_and_call_builder_and_error.CallBuilder
             erc20.erc20.Environment
             (ink_env.call.common.Set_
-              (ink_env.call.call_builder.Call erc20.erc20.Environment))
+              (ink_env.backend_and_call_builder_and_error.Call
+                erc20.erc20.Environment))
             (ink_env.call.common.Set_
               (ink_env.call.execution_input.ExecutionInput
                 (ink_env.call.execution_input.ArgumentList
@@ -4545,7 +4556,7 @@ Module Impl_erc20_erc20___CallBuilder_18.
                     ink_env.call.execution_input.EmptyArgumentList))))
             (ink_env.call.common.Set_
               (ink_env.call.common.ReturnType erc20.erc20.Balance))) :=
-    let* α0 := ink_env.call.call_builder.build_call in
+    let* α0 := ink_env.backend_and_call_builder_and_error.build_call in
     let* α1 := ink.contract_ref.ToAccountId.to_account_id self in
     let* α2 := α0.["call"] α1 in
     let* α3 := ink_env.call.selector.Selector::["new"] [ 106; 0; 22; 94 ] in
@@ -4567,10 +4578,11 @@ Module Impl_erc20_erc20___CallBuilder_18.
       (__ink_binding_1 : erc20.erc20.Balance)
       :
         M (H := H')
-          (ink_env.call.call_builder.CallBuilder
+          (ink_env.backend_and_call_builder_and_error.CallBuilder
             erc20.erc20.Environment
             (ink_env.call.common.Set_
-              (ink_env.call.call_builder.Call erc20.erc20.Environment))
+              (ink_env.backend_and_call_builder_and_error.Call
+                erc20.erc20.Environment))
             (ink_env.call.common.Set_
               (ink_env.call.execution_input.ExecutionInput
                 (ink_env.call.execution_input.ArgumentList
@@ -4581,7 +4593,7 @@ Module Impl_erc20_erc20___CallBuilder_18.
                     ink_env.call.execution_input.EmptyArgumentList))))
             (ink_env.call.common.Set_
               (ink_env.call.common.ReturnType (erc20.erc20.Result unit)))) :=
-    let* α0 := ink_env.call.call_builder.build_call in
+    let* α0 := ink_env.backend_and_call_builder_and_error.build_call in
     let* α1 := ink.contract_ref.ToAccountId.to_account_id self in
     let* α2 := α0.["call"] α1 in
     let* α3 := ink_env.call.selector.Selector::["new"] [ 132; 161; 93; 161 ] in
@@ -4603,10 +4615,11 @@ Module Impl_erc20_erc20___CallBuilder_18.
       (__ink_binding_1 : erc20.erc20.Balance)
       :
         M (H := H')
-          (ink_env.call.call_builder.CallBuilder
+          (ink_env.backend_and_call_builder_and_error.CallBuilder
             erc20.erc20.Environment
             (ink_env.call.common.Set_
-              (ink_env.call.call_builder.Call erc20.erc20.Environment))
+              (ink_env.backend_and_call_builder_and_error.Call
+                erc20.erc20.Environment))
             (ink_env.call.common.Set_
               (ink_env.call.execution_input.ExecutionInput
                 (ink_env.call.execution_input.ArgumentList
@@ -4617,7 +4630,7 @@ Module Impl_erc20_erc20___CallBuilder_18.
                     ink_env.call.execution_input.EmptyArgumentList))))
             (ink_env.call.common.Set_
               (ink_env.call.common.ReturnType (erc20.erc20.Result unit)))) :=
-    let* α0 := ink_env.call.call_builder.build_call in
+    let* α0 := ink_env.backend_and_call_builder_and_error.build_call in
     let* α1 := ink.contract_ref.ToAccountId.to_account_id self in
     let* α2 := α0.["call"] α1 in
     let* α3 := ink_env.call.selector.Selector::["new"] [ 104; 18; 102; 160 ] in
@@ -4640,10 +4653,11 @@ Module Impl_erc20_erc20___CallBuilder_18.
       (__ink_binding_2 : erc20.erc20.Balance)
       :
         M (H := H')
-          (ink_env.call.call_builder.CallBuilder
+          (ink_env.backend_and_call_builder_and_error.CallBuilder
             erc20.erc20.Environment
             (ink_env.call.common.Set_
-              (ink_env.call.call_builder.Call erc20.erc20.Environment))
+              (ink_env.backend_and_call_builder_and_error.Call
+                erc20.erc20.Environment))
             (ink_env.call.common.Set_
               (ink_env.call.execution_input.ExecutionInput
                 (ink_env.call.execution_input.ArgumentList
@@ -4657,7 +4671,7 @@ Module Impl_erc20_erc20___CallBuilder_18.
                       ink_env.call.execution_input.EmptyArgumentList)))))
             (ink_env.call.common.Set_
               (ink_env.call.common.ReturnType (erc20.erc20.Result unit)))) :=
-    let* α0 := ink_env.call.call_builder.build_call in
+    let* α0 := ink_env.backend_and_call_builder_and_error.build_call in
     let* α1 := ink.contract_ref.ToAccountId.to_account_id self in
     let* α2 := α0.["call"] α1 in
     let* α3 := ink_env.call.selector.Selector::["new"] [ 11; 57; 111; 24 ] in
